update the generated files
git-svn-id: https://projects.brucker.ch/hol-testgen/svn/HOL-TestGen/trunk/hol-testgen@11470 3260e6d1-4efc-4170-b0a7-36055960796d

doc/Employee_DesignModel_UMLPart_generated.thy
@@ -76,20 +76,20 @@ and implicitly of the class object. Each class implies the existence of a class
 type defined for the corresponding object representations as follows:  *}
 
 (* 14 ************************************ 13 + 8 *)
-datatype type\<^sub>P\<^sub>e\<^sub>r\<^sub>s\<^sub>o\<^sub>n = mk\<^sub>P\<^sub>e\<^sub>r\<^sub>s\<^sub>o\<^sub>n "oid" "nat option" "int option" "unit option" "bool option" "oid list list option"
-datatype typeoid\<^sub>P\<^sub>e\<^sub>r\<^sub>s\<^sub>o\<^sub>n = mkoid\<^sub>P\<^sub>e\<^sub>r\<^sub>s\<^sub>o\<^sub>n "type\<^sub>P\<^sub>e\<^sub>r\<^sub>s\<^sub>o\<^sub>n" "oid list option" "int option"
-datatype type\<^sub>P\<^sub>l\<^sub>a\<^sub>n\<^sub>e\<^sub>t = mk\<^sub>P\<^sub>l\<^sub>a\<^sub>n\<^sub>e\<^sub>t_\<^sub>P\<^sub>e\<^sub>r\<^sub>s\<^sub>o\<^sub>n "typeoid\<^sub>P\<^sub>e\<^sub>r\<^sub>s\<^sub>o\<^sub>n"
-                        | mk\<^sub>P\<^sub>l\<^sub>a\<^sub>n\<^sub>e\<^sub>t "oid" "unit option" "bool option" "oid list list option"
-datatype typeoid\<^sub>P\<^sub>l\<^sub>a\<^sub>n\<^sub>e\<^sub>t = mkoid\<^sub>P\<^sub>l\<^sub>a\<^sub>n\<^sub>e\<^sub>t "type\<^sub>P\<^sub>l\<^sub>a\<^sub>n\<^sub>e\<^sub>t" "nat option" "int option"
-datatype type\<^sub>G\<^sub>a\<^sub>l\<^sub>a\<^sub>x\<^sub>y = mk\<^sub>G\<^sub>a\<^sub>l\<^sub>a\<^sub>x\<^sub>y_\<^sub>P\<^sub>l\<^sub>a\<^sub>n\<^sub>e\<^sub>t "typeoid\<^sub>P\<^sub>l\<^sub>a\<^sub>n\<^sub>e\<^sub>t"
-                        | mk\<^sub>G\<^sub>a\<^sub>l\<^sub>a\<^sub>x\<^sub>y_\<^sub>P\<^sub>e\<^sub>r\<^sub>s\<^sub>o\<^sub>n "typeoid\<^sub>P\<^sub>e\<^sub>r\<^sub>s\<^sub>o\<^sub>n"
-                        | mk\<^sub>G\<^sub>a\<^sub>l\<^sub>a\<^sub>x\<^sub>y "oid"
-datatype typeoid\<^sub>G\<^sub>a\<^sub>l\<^sub>a\<^sub>x\<^sub>y = mkoid\<^sub>G\<^sub>a\<^sub>l\<^sub>a\<^sub>x\<^sub>y "type\<^sub>G\<^sub>a\<^sub>l\<^sub>a\<^sub>x\<^sub>y" "unit option" "bool option" "oid list list option"
-datatype type\<^sub>O\<^sub>c\<^sub>l\<^sub>A\<^sub>n\<^sub>y = mk\<^sub>O\<^sub>c\<^sub>l\<^sub>A\<^sub>n\<^sub>y_\<^sub>G\<^sub>a\<^sub>l\<^sub>a\<^sub>x\<^sub>y "typeoid\<^sub>G\<^sub>a\<^sub>l\<^sub>a\<^sub>x\<^sub>y"
-                        | mk\<^sub>O\<^sub>c\<^sub>l\<^sub>A\<^sub>n\<^sub>y_\<^sub>P\<^sub>l\<^sub>a\<^sub>n\<^sub>e\<^sub>t "typeoid\<^sub>P\<^sub>l\<^sub>a\<^sub>n\<^sub>e\<^sub>t"
-                        | mk\<^sub>O\<^sub>c\<^sub>l\<^sub>A\<^sub>n\<^sub>y_\<^sub>P\<^sub>e\<^sub>r\<^sub>s\<^sub>o\<^sub>n "typeoid\<^sub>P\<^sub>e\<^sub>r\<^sub>s\<^sub>o\<^sub>n"
-                        | mk\<^sub>O\<^sub>c\<^sub>l\<^sub>A\<^sub>n\<^sub>y "oid"
-datatype typeoid\<^sub>O\<^sub>c\<^sub>l\<^sub>A\<^sub>n\<^sub>y = mkoid\<^sub>O\<^sub>c\<^sub>l\<^sub>A\<^sub>n\<^sub>y "type\<^sub>O\<^sub>c\<^sub>l\<^sub>A\<^sub>n\<^sub>y"
+datatype ty\<E>\<X>\<T>\<^sub>P\<^sub>e\<^sub>r\<^sub>s\<^sub>o\<^sub>n = mk\<E>\<X>\<T>\<^sub>P\<^sub>e\<^sub>r\<^sub>s\<^sub>o\<^sub>n "oid" "nat option" "int option" "unit option" "bool option" "oid list list option"
+datatype ty\<^sub>P\<^sub>e\<^sub>r\<^sub>s\<^sub>o\<^sub>n = mk\<^sub>P\<^sub>e\<^sub>r\<^sub>s\<^sub>o\<^sub>n "ty\<E>\<X>\<T>\<^sub>P\<^sub>e\<^sub>r\<^sub>s\<^sub>o\<^sub>n" "oid list option" "int option"
+datatype ty\<E>\<X>\<T>\<^sub>P\<^sub>l\<^sub>a\<^sub>n\<^sub>e\<^sub>t = mk\<E>\<X>\<T>\<^sub>P\<^sub>l\<^sub>a\<^sub>n\<^sub>e\<^sub>t_\<^sub>P\<^sub>e\<^sub>r\<^sub>s\<^sub>o\<^sub>n "ty\<^sub>P\<^sub>e\<^sub>r\<^sub>s\<^sub>o\<^sub>n"
+                        | mk\<E>\<X>\<T>\<^sub>P\<^sub>l\<^sub>a\<^sub>n\<^sub>e\<^sub>t "oid" "unit option" "bool option" "oid list list option"
+datatype ty\<^sub>P\<^sub>l\<^sub>a\<^sub>n\<^sub>e\<^sub>t = mk\<^sub>P\<^sub>l\<^sub>a\<^sub>n\<^sub>e\<^sub>t "ty\<E>\<X>\<T>\<^sub>P\<^sub>l\<^sub>a\<^sub>n\<^sub>e\<^sub>t" "nat option" "int option"
+datatype ty\<E>\<X>\<T>\<^sub>G\<^sub>a\<^sub>l\<^sub>a\<^sub>x\<^sub>y = mk\<E>\<X>\<T>\<^sub>G\<^sub>a\<^sub>l\<^sub>a\<^sub>x\<^sub>y_\<^sub>P\<^sub>l\<^sub>a\<^sub>n\<^sub>e\<^sub>t "ty\<^sub>P\<^sub>l\<^sub>a\<^sub>n\<^sub>e\<^sub>t"
+                        | mk\<E>\<X>\<T>\<^sub>G\<^sub>a\<^sub>l\<^sub>a\<^sub>x\<^sub>y_\<^sub>P\<^sub>e\<^sub>r\<^sub>s\<^sub>o\<^sub>n "ty\<^sub>P\<^sub>e\<^sub>r\<^sub>s\<^sub>o\<^sub>n"
+                        | mk\<E>\<X>\<T>\<^sub>G\<^sub>a\<^sub>l\<^sub>a\<^sub>x\<^sub>y "oid"
+datatype ty\<^sub>G\<^sub>a\<^sub>l\<^sub>a\<^sub>x\<^sub>y = mk\<^sub>G\<^sub>a\<^sub>l\<^sub>a\<^sub>x\<^sub>y "ty\<E>\<X>\<T>\<^sub>G\<^sub>a\<^sub>l\<^sub>a\<^sub>x\<^sub>y" "unit option" "bool option" "oid list list option"
+datatype ty\<E>\<X>\<T>\<^sub>O\<^sub>c\<^sub>l\<^sub>A\<^sub>n\<^sub>y = mk\<E>\<X>\<T>\<^sub>O\<^sub>c\<^sub>l\<^sub>A\<^sub>n\<^sub>y_\<^sub>G\<^sub>a\<^sub>l\<^sub>a\<^sub>x\<^sub>y "ty\<^sub>G\<^sub>a\<^sub>l\<^sub>a\<^sub>x\<^sub>y"
+                        | mk\<E>\<X>\<T>\<^sub>O\<^sub>c\<^sub>l\<^sub>A\<^sub>n\<^sub>y_\<^sub>P\<^sub>l\<^sub>a\<^sub>n\<^sub>e\<^sub>t "ty\<^sub>P\<^sub>l\<^sub>a\<^sub>n\<^sub>e\<^sub>t"
+                        | mk\<E>\<X>\<T>\<^sub>O\<^sub>c\<^sub>l\<^sub>A\<^sub>n\<^sub>y_\<^sub>P\<^sub>e\<^sub>r\<^sub>s\<^sub>o\<^sub>n "ty\<^sub>P\<^sub>e\<^sub>r\<^sub>s\<^sub>o\<^sub>n"
+                        | mk\<E>\<X>\<T>\<^sub>O\<^sub>c\<^sub>l\<^sub>A\<^sub>n\<^sub>y "oid"
+datatype ty\<^sub>O\<^sub>c\<^sub>l\<^sub>A\<^sub>n\<^sub>y = mk\<^sub>O\<^sub>c\<^sub>l\<^sub>A\<^sub>n\<^sub>y "ty\<E>\<X>\<T>\<^sub>O\<^sub>c\<^sub>l\<^sub>A\<^sub>n\<^sub>y"
 
 (* 15 ************************************ 21 + 1 *)
 text{* 
@@ -98,10 +98,10 @@ sum type containing the class types. This type of OclAny will be used as instanc
 for all respective type-variables.  *}
 
 (* 16 ************************************ 22 + 1 *)
-datatype \<AA> = in\<^sub>P\<^sub>e\<^sub>r\<^sub>s\<^sub>o\<^sub>n "typeoid\<^sub>P\<^sub>e\<^sub>r\<^sub>s\<^sub>o\<^sub>n"
-                        | in\<^sub>P\<^sub>l\<^sub>a\<^sub>n\<^sub>e\<^sub>t "typeoid\<^sub>P\<^sub>l\<^sub>a\<^sub>n\<^sub>e\<^sub>t"
-                        | in\<^sub>G\<^sub>a\<^sub>l\<^sub>a\<^sub>x\<^sub>y "typeoid\<^sub>G\<^sub>a\<^sub>l\<^sub>a\<^sub>x\<^sub>y"
-                        | in\<^sub>O\<^sub>c\<^sub>l\<^sub>A\<^sub>n\<^sub>y "typeoid\<^sub>O\<^sub>c\<^sub>l\<^sub>A\<^sub>n\<^sub>y"
+datatype \<AA> = in\<^sub>P\<^sub>e\<^sub>r\<^sub>s\<^sub>o\<^sub>n "ty\<^sub>P\<^sub>e\<^sub>r\<^sub>s\<^sub>o\<^sub>n"
+                        | in\<^sub>P\<^sub>l\<^sub>a\<^sub>n\<^sub>e\<^sub>t "ty\<^sub>P\<^sub>l\<^sub>a\<^sub>n\<^sub>e\<^sub>t"
+                        | in\<^sub>G\<^sub>a\<^sub>l\<^sub>a\<^sub>x\<^sub>y "ty\<^sub>G\<^sub>a\<^sub>l\<^sub>a\<^sub>x\<^sub>y"
+                        | in\<^sub>O\<^sub>c\<^sub>l\<^sub>A\<^sub>n\<^sub>y "ty\<^sub>O\<^sub>c\<^sub>l\<^sub>A\<^sub>n\<^sub>y"
 
 (* 17 ************************************ 23 + 1 *)
 text{* 
@@ -115,15 +115,15 @@ type_synonym Boolean = "\<AA> Boolean"
 type_synonym Integer = "\<AA> Integer"
 type_synonym Real = "\<AA> Real"
 type_synonym String = "\<AA> String"
-type_synonym Person = "(\<AA>, typeoid\<^sub>P\<^sub>e\<^sub>r\<^sub>s\<^sub>o\<^sub>n option option) val"
-type_synonym Planet = "(\<AA>, typeoid\<^sub>P\<^sub>l\<^sub>a\<^sub>n\<^sub>e\<^sub>t option option) val"
-type_synonym Galaxy = "(\<AA>, typeoid\<^sub>G\<^sub>a\<^sub>l\<^sub>a\<^sub>x\<^sub>y option option) val"
-type_synonym OclAny = "(\<AA>, typeoid\<^sub>O\<^sub>c\<^sub>l\<^sub>A\<^sub>n\<^sub>y option option) val"
+type_synonym Person = "(\<AA>, ty\<^sub>P\<^sub>e\<^sub>r\<^sub>s\<^sub>o\<^sub>n option option) val"
+type_synonym Planet = "(\<AA>, ty\<^sub>P\<^sub>l\<^sub>a\<^sub>n\<^sub>e\<^sub>t option option) val"
+type_synonym Galaxy = "(\<AA>, ty\<^sub>G\<^sub>a\<^sub>l\<^sub>a\<^sub>x\<^sub>y option option) val"
+type_synonym OclAny = "(\<AA>, ty\<^sub>O\<^sub>c\<^sub>l\<^sub>A\<^sub>n\<^sub>y option option) val"
 
 (* 19 ************************************ 33 + 3 *)
-type_synonym Sequence_Person = "(\<AA>, typeoid\<^sub>P\<^sub>e\<^sub>r\<^sub>s\<^sub>o\<^sub>n option option Sequence\<^sub>b\<^sub>a\<^sub>s\<^sub>e) val"
-type_synonym Set_Person = "(\<AA>, typeoid\<^sub>P\<^sub>e\<^sub>r\<^sub>s\<^sub>o\<^sub>n option option Set\<^sub>b\<^sub>a\<^sub>s\<^sub>e) val"
-type_synonym Set_Sequence_Planet = "(\<AA>, typeoid\<^sub>P\<^sub>l\<^sub>a\<^sub>n\<^sub>e\<^sub>t option option Sequence\<^sub>b\<^sub>a\<^sub>s\<^sub>e Set\<^sub>b\<^sub>a\<^sub>s\<^sub>e) val"
+type_synonym Sequence_Person = "(\<AA>, ty\<^sub>P\<^sub>e\<^sub>r\<^sub>s\<^sub>o\<^sub>n option option Sequence\<^sub>b\<^sub>a\<^sub>s\<^sub>e) val"
+type_synonym Set_Person = "(\<AA>, ty\<^sub>P\<^sub>e\<^sub>r\<^sub>s\<^sub>o\<^sub>n option option Set\<^sub>b\<^sub>a\<^sub>s\<^sub>e) val"
+type_synonym Set_Sequence_Planet = "(\<AA>, ty\<^sub>P\<^sub>l\<^sub>a\<^sub>n\<^sub>e\<^sub>t option option Sequence\<^sub>b\<^sub>a\<^sub>s\<^sub>e Set\<^sub>b\<^sub>a\<^sub>s\<^sub>e) val"
 
 (* 20 ************************************ 36 + 1 *)
 text{* 
@@ -132,30 +132,30 @@ to show that the object universe belongs to the type class ``oclany,'' \ie,
  each class type has to provide a function @{term oid_of} yielding the object id (oid) of the object.  *}
 
 (* 21 ************************************ 37 + 4 *)
-instantiation typeoid\<^sub>P\<^sub>e\<^sub>r\<^sub>s\<^sub>o\<^sub>n :: object
+instantiation ty\<^sub>P\<^sub>e\<^sub>r\<^sub>s\<^sub>o\<^sub>n :: object
 begin
-  definition oid_of_typeoid\<^sub>P\<^sub>e\<^sub>r\<^sub>s\<^sub>o\<^sub>n_def : "oid_of = (\<lambda> mkoid\<^sub>P\<^sub>e\<^sub>r\<^sub>s\<^sub>o\<^sub>n t _ _ \<Rightarrow> (case t of (mk\<^sub>P\<^sub>e\<^sub>r\<^sub>s\<^sub>o\<^sub>n (t) (_) (_) (_) (_) (_)) \<Rightarrow> t))"
+  definition oid_of_ty\<^sub>P\<^sub>e\<^sub>r\<^sub>s\<^sub>o\<^sub>n_def : "oid_of = (\<lambda> mk\<^sub>P\<^sub>e\<^sub>r\<^sub>s\<^sub>o\<^sub>n t _ _ \<Rightarrow> (case t of (mk\<E>\<X>\<T>\<^sub>P\<^sub>e\<^sub>r\<^sub>s\<^sub>o\<^sub>n (t) (_) (_) (_) (_) (_)) \<Rightarrow> t))"
   instance ..
 end
-instantiation typeoid\<^sub>P\<^sub>l\<^sub>a\<^sub>n\<^sub>e\<^sub>t :: object
+instantiation ty\<^sub>P\<^sub>l\<^sub>a\<^sub>n\<^sub>e\<^sub>t :: object
 begin
-  definition oid_of_typeoid\<^sub>P\<^sub>l\<^sub>a\<^sub>n\<^sub>e\<^sub>t_def : "oid_of = (\<lambda> mkoid\<^sub>P\<^sub>l\<^sub>a\<^sub>n\<^sub>e\<^sub>t t _ _ \<Rightarrow> (case t of (mk\<^sub>P\<^sub>l\<^sub>a\<^sub>n\<^sub>e\<^sub>t (t) (_) (_) (_)) \<Rightarrow> t
-    | (mk\<^sub>P\<^sub>l\<^sub>a\<^sub>n\<^sub>e\<^sub>t_\<^sub>P\<^sub>e\<^sub>r\<^sub>s\<^sub>o\<^sub>n (t)) \<Rightarrow> (oid_of (t))))"
+  definition oid_of_ty\<^sub>P\<^sub>l\<^sub>a\<^sub>n\<^sub>e\<^sub>t_def : "oid_of = (\<lambda> mk\<^sub>P\<^sub>l\<^sub>a\<^sub>n\<^sub>e\<^sub>t t _ _ \<Rightarrow> (case t of (mk\<E>\<X>\<T>\<^sub>P\<^sub>l\<^sub>a\<^sub>n\<^sub>e\<^sub>t (t) (_) (_) (_)) \<Rightarrow> t
+    | (mk\<E>\<X>\<T>\<^sub>P\<^sub>l\<^sub>a\<^sub>n\<^sub>e\<^sub>t_\<^sub>P\<^sub>e\<^sub>r\<^sub>s\<^sub>o\<^sub>n (t)) \<Rightarrow> (oid_of (t))))"
   instance ..
 end
-instantiation typeoid\<^sub>G\<^sub>a\<^sub>l\<^sub>a\<^sub>x\<^sub>y :: object
+instantiation ty\<^sub>G\<^sub>a\<^sub>l\<^sub>a\<^sub>x\<^sub>y :: object
 begin
-  definition oid_of_typeoid\<^sub>G\<^sub>a\<^sub>l\<^sub>a\<^sub>x\<^sub>y_def : "oid_of = (\<lambda> mkoid\<^sub>G\<^sub>a\<^sub>l\<^sub>a\<^sub>x\<^sub>y t _ _ _ \<Rightarrow> (case t of (mk\<^sub>G\<^sub>a\<^sub>l\<^sub>a\<^sub>x\<^sub>y (t)) \<Rightarrow> t
-    | (mk\<^sub>G\<^sub>a\<^sub>l\<^sub>a\<^sub>x\<^sub>y_\<^sub>P\<^sub>e\<^sub>r\<^sub>s\<^sub>o\<^sub>n (t)) \<Rightarrow> (oid_of (t))
-    | (mk\<^sub>G\<^sub>a\<^sub>l\<^sub>a\<^sub>x\<^sub>y_\<^sub>P\<^sub>l\<^sub>a\<^sub>n\<^sub>e\<^sub>t (t)) \<Rightarrow> (oid_of (t))))"
+  definition oid_of_ty\<^sub>G\<^sub>a\<^sub>l\<^sub>a\<^sub>x\<^sub>y_def : "oid_of = (\<lambda> mk\<^sub>G\<^sub>a\<^sub>l\<^sub>a\<^sub>x\<^sub>y t _ _ _ \<Rightarrow> (case t of (mk\<E>\<X>\<T>\<^sub>G\<^sub>a\<^sub>l\<^sub>a\<^sub>x\<^sub>y (t)) \<Rightarrow> t
+    | (mk\<E>\<X>\<T>\<^sub>G\<^sub>a\<^sub>l\<^sub>a\<^sub>x\<^sub>y_\<^sub>P\<^sub>e\<^sub>r\<^sub>s\<^sub>o\<^sub>n (t)) \<Rightarrow> (oid_of (t))
+    | (mk\<E>\<X>\<T>\<^sub>G\<^sub>a\<^sub>l\<^sub>a\<^sub>x\<^sub>y_\<^sub>P\<^sub>l\<^sub>a\<^sub>n\<^sub>e\<^sub>t (t)) \<Rightarrow> (oid_of (t))))"
   instance ..
 end
-instantiation typeoid\<^sub>O\<^sub>c\<^sub>l\<^sub>A\<^sub>n\<^sub>y :: object
+instantiation ty\<^sub>O\<^sub>c\<^sub>l\<^sub>A\<^sub>n\<^sub>y :: object
 begin
-  definition oid_of_typeoid\<^sub>O\<^sub>c\<^sub>l\<^sub>A\<^sub>n\<^sub>y_def : "oid_of = (\<lambda> mkoid\<^sub>O\<^sub>c\<^sub>l\<^sub>A\<^sub>n\<^sub>y t \<Rightarrow> (case t of (mk\<^sub>O\<^sub>c\<^sub>l\<^sub>A\<^sub>n\<^sub>y (t)) \<Rightarrow> t
-    | (mk\<^sub>O\<^sub>c\<^sub>l\<^sub>A\<^sub>n\<^sub>y_\<^sub>P\<^sub>e\<^sub>r\<^sub>s\<^sub>o\<^sub>n (t)) \<Rightarrow> (oid_of (t))
-    | (mk\<^sub>O\<^sub>c\<^sub>l\<^sub>A\<^sub>n\<^sub>y_\<^sub>P\<^sub>l\<^sub>a\<^sub>n\<^sub>e\<^sub>t (t)) \<Rightarrow> (oid_of (t))
-    | (mk\<^sub>O\<^sub>c\<^sub>l\<^sub>A\<^sub>n\<^sub>y_\<^sub>G\<^sub>a\<^sub>l\<^sub>a\<^sub>x\<^sub>y (t)) \<Rightarrow> (oid_of (t))))"
+  definition oid_of_ty\<^sub>O\<^sub>c\<^sub>l\<^sub>A\<^sub>n\<^sub>y_def : "oid_of = (\<lambda> mk\<^sub>O\<^sub>c\<^sub>l\<^sub>A\<^sub>n\<^sub>y t \<Rightarrow> (case t of (mk\<E>\<X>\<T>\<^sub>O\<^sub>c\<^sub>l\<^sub>A\<^sub>n\<^sub>y (t)) \<Rightarrow> t
+    | (mk\<E>\<X>\<T>\<^sub>O\<^sub>c\<^sub>l\<^sub>A\<^sub>n\<^sub>y_\<^sub>P\<^sub>e\<^sub>r\<^sub>s\<^sub>o\<^sub>n (t)) \<Rightarrow> (oid_of (t))
+    | (mk\<E>\<X>\<T>\<^sub>O\<^sub>c\<^sub>l\<^sub>A\<^sub>n\<^sub>y_\<^sub>P\<^sub>l\<^sub>a\<^sub>n\<^sub>e\<^sub>t (t)) \<Rightarrow> (oid_of (t))
+    | (mk\<E>\<X>\<T>\<^sub>O\<^sub>c\<^sub>l\<^sub>A\<^sub>n\<^sub>y_\<^sub>G\<^sub>a\<^sub>l\<^sub>a\<^sub>x\<^sub>y (t)) \<Rightarrow> (oid_of (t))))"
   instance ..
 end
 
@@ -218,70 +218,70 @@ consts OclAsType\<^sub>O\<^sub>c\<^sub>l\<^sub>A\<^sub>n\<^sub>y :: "'\<alpha> \
 defs(overloaded) OclAsType\<^sub>P\<^sub>e\<^sub>r\<^sub>s\<^sub>o\<^sub>n_Person : "(x::Person) .oclAsType(Person) \<equiv> x"
 defs(overloaded) OclAsType\<^sub>P\<^sub>e\<^sub>r\<^sub>s\<^sub>o\<^sub>n_Planet : "(x::Planet) .oclAsType(Person) \<equiv> (\<lambda>\<tau>. (case (x (\<tau>)) of \<bottom> \<Rightarrow> (invalid (\<tau>))
     | \<lfloor>\<bottom>\<rfloor> \<Rightarrow> (null (\<tau>))
-    | \<lfloor>\<lfloor>(mkoid\<^sub>P\<^sub>l\<^sub>a\<^sub>n\<^sub>e\<^sub>t ((mk\<^sub>P\<^sub>l\<^sub>a\<^sub>n\<^sub>e\<^sub>t_\<^sub>P\<^sub>e\<^sub>r\<^sub>s\<^sub>o\<^sub>n (Person))) (_) (_))\<rfloor>\<rfloor> \<Rightarrow> \<lfloor>\<lfloor>Person\<rfloor>\<rfloor>
+    | \<lfloor>\<lfloor>(mk\<^sub>P\<^sub>l\<^sub>a\<^sub>n\<^sub>e\<^sub>t ((mk\<E>\<X>\<T>\<^sub>P\<^sub>l\<^sub>a\<^sub>n\<^sub>e\<^sub>t_\<^sub>P\<^sub>e\<^sub>r\<^sub>s\<^sub>o\<^sub>n (Person))) (_) (_))\<rfloor>\<rfloor> \<Rightarrow> \<lfloor>\<lfloor>Person\<rfloor>\<rfloor>
     | _ \<Rightarrow> (invalid (\<tau>))))"
 defs(overloaded) OclAsType\<^sub>P\<^sub>e\<^sub>r\<^sub>s\<^sub>o\<^sub>n_Galaxy : "(x::Galaxy) .oclAsType(Person) \<equiv> (\<lambda>\<tau>. (case (x (\<tau>)) of \<bottom> \<Rightarrow> (invalid (\<tau>))
     | \<lfloor>\<bottom>\<rfloor> \<Rightarrow> (null (\<tau>))
-    | \<lfloor>\<lfloor>(mkoid\<^sub>G\<^sub>a\<^sub>l\<^sub>a\<^sub>x\<^sub>y ((mk\<^sub>G\<^sub>a\<^sub>l\<^sub>a\<^sub>x\<^sub>y_\<^sub>P\<^sub>e\<^sub>r\<^sub>s\<^sub>o\<^sub>n (Person))) (_) (_) (_))\<rfloor>\<rfloor> \<Rightarrow> \<lfloor>\<lfloor>Person\<rfloor>\<rfloor>
+    | \<lfloor>\<lfloor>(mk\<^sub>G\<^sub>a\<^sub>l\<^sub>a\<^sub>x\<^sub>y ((mk\<E>\<X>\<T>\<^sub>G\<^sub>a\<^sub>l\<^sub>a\<^sub>x\<^sub>y_\<^sub>P\<^sub>e\<^sub>r\<^sub>s\<^sub>o\<^sub>n (Person))) (_) (_) (_))\<rfloor>\<rfloor> \<Rightarrow> \<lfloor>\<lfloor>Person\<rfloor>\<rfloor>
     | _ \<Rightarrow> (invalid (\<tau>))))"
 defs(overloaded) OclAsType\<^sub>P\<^sub>e\<^sub>r\<^sub>s\<^sub>o\<^sub>n_OclAny : "(x::OclAny) .oclAsType(Person) \<equiv> (\<lambda>\<tau>. (case (x (\<tau>)) of \<bottom> \<Rightarrow> (invalid (\<tau>))
     | \<lfloor>\<bottom>\<rfloor> \<Rightarrow> (null (\<tau>))
-    | \<lfloor>\<lfloor>(mkoid\<^sub>O\<^sub>c\<^sub>l\<^sub>A\<^sub>n\<^sub>y ((mk\<^sub>O\<^sub>c\<^sub>l\<^sub>A\<^sub>n\<^sub>y_\<^sub>P\<^sub>e\<^sub>r\<^sub>s\<^sub>o\<^sub>n (Person))))\<rfloor>\<rfloor> \<Rightarrow> \<lfloor>\<lfloor>Person\<rfloor>\<rfloor>
+    | \<lfloor>\<lfloor>(mk\<^sub>O\<^sub>c\<^sub>l\<^sub>A\<^sub>n\<^sub>y ((mk\<E>\<X>\<T>\<^sub>O\<^sub>c\<^sub>l\<^sub>A\<^sub>n\<^sub>y_\<^sub>P\<^sub>e\<^sub>r\<^sub>s\<^sub>o\<^sub>n (Person))))\<rfloor>\<rfloor> \<Rightarrow> \<lfloor>\<lfloor>Person\<rfloor>\<rfloor>
     | _ \<Rightarrow> (invalid (\<tau>))))"
 defs(overloaded) OclAsType\<^sub>P\<^sub>l\<^sub>a\<^sub>n\<^sub>e\<^sub>t_Planet : "(x::Planet) .oclAsType(Planet) \<equiv> x"
 defs(overloaded) OclAsType\<^sub>P\<^sub>l\<^sub>a\<^sub>n\<^sub>e\<^sub>t_Galaxy : "(x::Galaxy) .oclAsType(Planet) \<equiv> (\<lambda>\<tau>. (case (x (\<tau>)) of \<bottom> \<Rightarrow> (invalid (\<tau>))
     | \<lfloor>\<bottom>\<rfloor> \<Rightarrow> (null (\<tau>))
-    | \<lfloor>\<lfloor>(mkoid\<^sub>G\<^sub>a\<^sub>l\<^sub>a\<^sub>x\<^sub>y ((mk\<^sub>G\<^sub>a\<^sub>l\<^sub>a\<^sub>x\<^sub>y_\<^sub>P\<^sub>l\<^sub>a\<^sub>n\<^sub>e\<^sub>t (Planet))) (_) (_) (_))\<rfloor>\<rfloor> \<Rightarrow> \<lfloor>\<lfloor>Planet\<rfloor>\<rfloor>
+    | \<lfloor>\<lfloor>(mk\<^sub>G\<^sub>a\<^sub>l\<^sub>a\<^sub>x\<^sub>y ((mk\<E>\<X>\<T>\<^sub>G\<^sub>a\<^sub>l\<^sub>a\<^sub>x\<^sub>y_\<^sub>P\<^sub>l\<^sub>a\<^sub>n\<^sub>e\<^sub>t (Planet))) (_) (_) (_))\<rfloor>\<rfloor> \<Rightarrow> \<lfloor>\<lfloor>Planet\<rfloor>\<rfloor>
     | _ \<Rightarrow> (invalid (\<tau>))))"
 defs(overloaded) OclAsType\<^sub>P\<^sub>l\<^sub>a\<^sub>n\<^sub>e\<^sub>t_OclAny : "(x::OclAny) .oclAsType(Planet) \<equiv> (\<lambda>\<tau>. (case (x (\<tau>)) of \<bottom> \<Rightarrow> (invalid (\<tau>))
     | \<lfloor>\<bottom>\<rfloor> \<Rightarrow> (null (\<tau>))
-    | \<lfloor>\<lfloor>(mkoid\<^sub>O\<^sub>c\<^sub>l\<^sub>A\<^sub>n\<^sub>y ((mk\<^sub>O\<^sub>c\<^sub>l\<^sub>A\<^sub>n\<^sub>y_\<^sub>P\<^sub>l\<^sub>a\<^sub>n\<^sub>e\<^sub>t (Planet))))\<rfloor>\<rfloor> \<Rightarrow> \<lfloor>\<lfloor>Planet\<rfloor>\<rfloor>
+    | \<lfloor>\<lfloor>(mk\<^sub>O\<^sub>c\<^sub>l\<^sub>A\<^sub>n\<^sub>y ((mk\<E>\<X>\<T>\<^sub>O\<^sub>c\<^sub>l\<^sub>A\<^sub>n\<^sub>y_\<^sub>P\<^sub>l\<^sub>a\<^sub>n\<^sub>e\<^sub>t (Planet))))\<rfloor>\<rfloor> \<Rightarrow> \<lfloor>\<lfloor>Planet\<rfloor>\<rfloor>
     | _ \<Rightarrow> (invalid (\<tau>))))"
 defs(overloaded) OclAsType\<^sub>P\<^sub>l\<^sub>a\<^sub>n\<^sub>e\<^sub>t_Person : "(x::Person) .oclAsType(Planet) \<equiv> (\<lambda>\<tau>. (case (x (\<tau>)) of \<bottom> \<Rightarrow> (invalid (\<tau>))
     | \<lfloor>\<bottom>\<rfloor> \<Rightarrow> (null (\<tau>))
-    | \<lfloor>\<lfloor>Person\<rfloor>\<rfloor> \<Rightarrow> \<lfloor>\<lfloor>(mkoid\<^sub>P\<^sub>l\<^sub>a\<^sub>n\<^sub>e\<^sub>t ((mk\<^sub>P\<^sub>l\<^sub>a\<^sub>n\<^sub>e\<^sub>t_\<^sub>P\<^sub>e\<^sub>r\<^sub>s\<^sub>o\<^sub>n (Person))) (None) (None))\<rfloor>\<rfloor>))"
+    | \<lfloor>\<lfloor>Person\<rfloor>\<rfloor> \<Rightarrow> \<lfloor>\<lfloor>(mk\<^sub>P\<^sub>l\<^sub>a\<^sub>n\<^sub>e\<^sub>t ((mk\<E>\<X>\<T>\<^sub>P\<^sub>l\<^sub>a\<^sub>n\<^sub>e\<^sub>t_\<^sub>P\<^sub>e\<^sub>r\<^sub>s\<^sub>o\<^sub>n (Person))) (None) (None))\<rfloor>\<rfloor>))"
 defs(overloaded) OclAsType\<^sub>G\<^sub>a\<^sub>l\<^sub>a\<^sub>x\<^sub>y_Galaxy : "(x::Galaxy) .oclAsType(Galaxy) \<equiv> x"
 defs(overloaded) OclAsType\<^sub>G\<^sub>a\<^sub>l\<^sub>a\<^sub>x\<^sub>y_OclAny : "(x::OclAny) .oclAsType(Galaxy) \<equiv> (\<lambda>\<tau>. (case (x (\<tau>)) of \<bottom> \<Rightarrow> (invalid (\<tau>))
     | \<lfloor>\<bottom>\<rfloor> \<Rightarrow> (null (\<tau>))
-    | \<lfloor>\<lfloor>(mkoid\<^sub>O\<^sub>c\<^sub>l\<^sub>A\<^sub>n\<^sub>y ((mk\<^sub>O\<^sub>c\<^sub>l\<^sub>A\<^sub>n\<^sub>y_\<^sub>G\<^sub>a\<^sub>l\<^sub>a\<^sub>x\<^sub>y (Galaxy))))\<rfloor>\<rfloor> \<Rightarrow> \<lfloor>\<lfloor>Galaxy\<rfloor>\<rfloor>
+    | \<lfloor>\<lfloor>(mk\<^sub>O\<^sub>c\<^sub>l\<^sub>A\<^sub>n\<^sub>y ((mk\<E>\<X>\<T>\<^sub>O\<^sub>c\<^sub>l\<^sub>A\<^sub>n\<^sub>y_\<^sub>G\<^sub>a\<^sub>l\<^sub>a\<^sub>x\<^sub>y (Galaxy))))\<rfloor>\<rfloor> \<Rightarrow> \<lfloor>\<lfloor>Galaxy\<rfloor>\<rfloor>
     | _ \<Rightarrow> (invalid (\<tau>))))"
 defs(overloaded) OclAsType\<^sub>G\<^sub>a\<^sub>l\<^sub>a\<^sub>x\<^sub>y_Person : "(x::Person) .oclAsType(Galaxy) \<equiv> (\<lambda>\<tau>. (case (x (\<tau>)) of \<bottom> \<Rightarrow> (invalid (\<tau>))
     | \<lfloor>\<bottom>\<rfloor> \<Rightarrow> (null (\<tau>))
-    | \<lfloor>\<lfloor>Person\<rfloor>\<rfloor> \<Rightarrow> \<lfloor>\<lfloor>(mkoid\<^sub>G\<^sub>a\<^sub>l\<^sub>a\<^sub>x\<^sub>y ((mk\<^sub>G\<^sub>a\<^sub>l\<^sub>a\<^sub>x\<^sub>y_\<^sub>P\<^sub>e\<^sub>r\<^sub>s\<^sub>o\<^sub>n (Person))) (None) (None) (None))\<rfloor>\<rfloor>))"
+    | \<lfloor>\<lfloor>Person\<rfloor>\<rfloor> \<Rightarrow> \<lfloor>\<lfloor>(mk\<^sub>G\<^sub>a\<^sub>l\<^sub>a\<^sub>x\<^sub>y ((mk\<E>\<X>\<T>\<^sub>G\<^sub>a\<^sub>l\<^sub>a\<^sub>x\<^sub>y_\<^sub>P\<^sub>e\<^sub>r\<^sub>s\<^sub>o\<^sub>n (Person))) (None) (None) (None))\<rfloor>\<rfloor>))"
 defs(overloaded) OclAsType\<^sub>G\<^sub>a\<^sub>l\<^sub>a\<^sub>x\<^sub>y_Planet : "(x::Planet) .oclAsType(Galaxy) \<equiv> (\<lambda>\<tau>. (case (x (\<tau>)) of \<bottom> \<Rightarrow> (invalid (\<tau>))
     | \<lfloor>\<bottom>\<rfloor> \<Rightarrow> (null (\<tau>))
-    | \<lfloor>\<lfloor>Planet\<rfloor>\<rfloor> \<Rightarrow> \<lfloor>\<lfloor>(mkoid\<^sub>G\<^sub>a\<^sub>l\<^sub>a\<^sub>x\<^sub>y ((mk\<^sub>G\<^sub>a\<^sub>l\<^sub>a\<^sub>x\<^sub>y_\<^sub>P\<^sub>l\<^sub>a\<^sub>n\<^sub>e\<^sub>t (Planet))) (None) (None) (None))\<rfloor>\<rfloor>))"
+    | \<lfloor>\<lfloor>Planet\<rfloor>\<rfloor> \<Rightarrow> \<lfloor>\<lfloor>(mk\<^sub>G\<^sub>a\<^sub>l\<^sub>a\<^sub>x\<^sub>y ((mk\<E>\<X>\<T>\<^sub>G\<^sub>a\<^sub>l\<^sub>a\<^sub>x\<^sub>y_\<^sub>P\<^sub>l\<^sub>a\<^sub>n\<^sub>e\<^sub>t (Planet))) (None) (None) (None))\<rfloor>\<rfloor>))"
 defs(overloaded) OclAsType\<^sub>O\<^sub>c\<^sub>l\<^sub>A\<^sub>n\<^sub>y_OclAny : "(x::OclAny) .oclAsType(OclAny) \<equiv> x"
 defs(overloaded) OclAsType\<^sub>O\<^sub>c\<^sub>l\<^sub>A\<^sub>n\<^sub>y_Person : "(x::Person) .oclAsType(OclAny) \<equiv> (\<lambda>\<tau>. (case (x (\<tau>)) of \<bottom> \<Rightarrow> (invalid (\<tau>))
     | \<lfloor>\<bottom>\<rfloor> \<Rightarrow> (null (\<tau>))
-    | \<lfloor>\<lfloor>Person\<rfloor>\<rfloor> \<Rightarrow> \<lfloor>\<lfloor>(mkoid\<^sub>O\<^sub>c\<^sub>l\<^sub>A\<^sub>n\<^sub>y ((mk\<^sub>O\<^sub>c\<^sub>l\<^sub>A\<^sub>n\<^sub>y_\<^sub>P\<^sub>e\<^sub>r\<^sub>s\<^sub>o\<^sub>n (Person))))\<rfloor>\<rfloor>))"
+    | \<lfloor>\<lfloor>Person\<rfloor>\<rfloor> \<Rightarrow> \<lfloor>\<lfloor>(mk\<^sub>O\<^sub>c\<^sub>l\<^sub>A\<^sub>n\<^sub>y ((mk\<E>\<X>\<T>\<^sub>O\<^sub>c\<^sub>l\<^sub>A\<^sub>n\<^sub>y_\<^sub>P\<^sub>e\<^sub>r\<^sub>s\<^sub>o\<^sub>n (Person))))\<rfloor>\<rfloor>))"
 defs(overloaded) OclAsType\<^sub>O\<^sub>c\<^sub>l\<^sub>A\<^sub>n\<^sub>y_Planet : "(x::Planet) .oclAsType(OclAny) \<equiv> (\<lambda>\<tau>. (case (x (\<tau>)) of \<bottom> \<Rightarrow> (invalid (\<tau>))
     | \<lfloor>\<bottom>\<rfloor> \<Rightarrow> (null (\<tau>))
-    | \<lfloor>\<lfloor>Planet\<rfloor>\<rfloor> \<Rightarrow> \<lfloor>\<lfloor>(mkoid\<^sub>O\<^sub>c\<^sub>l\<^sub>A\<^sub>n\<^sub>y ((mk\<^sub>O\<^sub>c\<^sub>l\<^sub>A\<^sub>n\<^sub>y_\<^sub>P\<^sub>l\<^sub>a\<^sub>n\<^sub>e\<^sub>t (Planet))))\<rfloor>\<rfloor>))"
+    | \<lfloor>\<lfloor>Planet\<rfloor>\<rfloor> \<Rightarrow> \<lfloor>\<lfloor>(mk\<^sub>O\<^sub>c\<^sub>l\<^sub>A\<^sub>n\<^sub>y ((mk\<E>\<X>\<T>\<^sub>O\<^sub>c\<^sub>l\<^sub>A\<^sub>n\<^sub>y_\<^sub>P\<^sub>l\<^sub>a\<^sub>n\<^sub>e\<^sub>t (Planet))))\<rfloor>\<rfloor>))"
 defs(overloaded) OclAsType\<^sub>O\<^sub>c\<^sub>l\<^sub>A\<^sub>n\<^sub>y_Galaxy : "(x::Galaxy) .oclAsType(OclAny) \<equiv> (\<lambda>\<tau>. (case (x (\<tau>)) of \<bottom> \<Rightarrow> (invalid (\<tau>))
     | \<lfloor>\<bottom>\<rfloor> \<Rightarrow> (null (\<tau>))
-    | \<lfloor>\<lfloor>Galaxy\<rfloor>\<rfloor> \<Rightarrow> \<lfloor>\<lfloor>(mkoid\<^sub>O\<^sub>c\<^sub>l\<^sub>A\<^sub>n\<^sub>y ((mk\<^sub>O\<^sub>c\<^sub>l\<^sub>A\<^sub>n\<^sub>y_\<^sub>G\<^sub>a\<^sub>l\<^sub>a\<^sub>x\<^sub>y (Galaxy))))\<rfloor>\<rfloor>))"
+    | \<lfloor>\<lfloor>Galaxy\<rfloor>\<rfloor> \<Rightarrow> \<lfloor>\<lfloor>(mk\<^sub>O\<^sub>c\<^sub>l\<^sub>A\<^sub>n\<^sub>y ((mk\<E>\<X>\<T>\<^sub>O\<^sub>c\<^sub>l\<^sub>A\<^sub>n\<^sub>y_\<^sub>G\<^sub>a\<^sub>l\<^sub>a\<^sub>x\<^sub>y (Galaxy))))\<rfloor>\<rfloor>))"
 
 (* 33 ************************************ 73 + 4 *)
 definition "OclAsType\<^sub>P\<^sub>e\<^sub>r\<^sub>s\<^sub>o\<^sub>n_\<AA> = (\<lambda> (in\<^sub>P\<^sub>e\<^sub>r\<^sub>s\<^sub>o\<^sub>n (Person)) \<Rightarrow> \<lfloor>Person\<rfloor>
-    | (in\<^sub>P\<^sub>l\<^sub>a\<^sub>n\<^sub>e\<^sub>t ((mkoid\<^sub>P\<^sub>l\<^sub>a\<^sub>n\<^sub>e\<^sub>t ((mk\<^sub>P\<^sub>l\<^sub>a\<^sub>n\<^sub>e\<^sub>t_\<^sub>P\<^sub>e\<^sub>r\<^sub>s\<^sub>o\<^sub>n (Person))) (_) (_)))) \<Rightarrow> \<lfloor>Person\<rfloor>
-    | (in\<^sub>G\<^sub>a\<^sub>l\<^sub>a\<^sub>x\<^sub>y ((mkoid\<^sub>G\<^sub>a\<^sub>l\<^sub>a\<^sub>x\<^sub>y ((mk\<^sub>G\<^sub>a\<^sub>l\<^sub>a\<^sub>x\<^sub>y_\<^sub>P\<^sub>e\<^sub>r\<^sub>s\<^sub>o\<^sub>n (Person))) (_) (_) (_)))) \<Rightarrow> \<lfloor>Person\<rfloor>
-    | (in\<^sub>O\<^sub>c\<^sub>l\<^sub>A\<^sub>n\<^sub>y ((mkoid\<^sub>O\<^sub>c\<^sub>l\<^sub>A\<^sub>n\<^sub>y ((mk\<^sub>O\<^sub>c\<^sub>l\<^sub>A\<^sub>n\<^sub>y_\<^sub>P\<^sub>e\<^sub>r\<^sub>s\<^sub>o\<^sub>n (Person)))))) \<Rightarrow> \<lfloor>Person\<rfloor>
+    | (in\<^sub>P\<^sub>l\<^sub>a\<^sub>n\<^sub>e\<^sub>t ((mk\<^sub>P\<^sub>l\<^sub>a\<^sub>n\<^sub>e\<^sub>t ((mk\<E>\<X>\<T>\<^sub>P\<^sub>l\<^sub>a\<^sub>n\<^sub>e\<^sub>t_\<^sub>P\<^sub>e\<^sub>r\<^sub>s\<^sub>o\<^sub>n (Person))) (_) (_)))) \<Rightarrow> \<lfloor>Person\<rfloor>
+    | (in\<^sub>G\<^sub>a\<^sub>l\<^sub>a\<^sub>x\<^sub>y ((mk\<^sub>G\<^sub>a\<^sub>l\<^sub>a\<^sub>x\<^sub>y ((mk\<E>\<X>\<T>\<^sub>G\<^sub>a\<^sub>l\<^sub>a\<^sub>x\<^sub>y_\<^sub>P\<^sub>e\<^sub>r\<^sub>s\<^sub>o\<^sub>n (Person))) (_) (_) (_)))) \<Rightarrow> \<lfloor>Person\<rfloor>
+    | (in\<^sub>O\<^sub>c\<^sub>l\<^sub>A\<^sub>n\<^sub>y ((mk\<^sub>O\<^sub>c\<^sub>l\<^sub>A\<^sub>n\<^sub>y ((mk\<E>\<X>\<T>\<^sub>O\<^sub>c\<^sub>l\<^sub>A\<^sub>n\<^sub>y_\<^sub>P\<^sub>e\<^sub>r\<^sub>s\<^sub>o\<^sub>n (Person)))))) \<Rightarrow> \<lfloor>Person\<rfloor>
     | _ \<Rightarrow> None)"
 definition "OclAsType\<^sub>P\<^sub>l\<^sub>a\<^sub>n\<^sub>e\<^sub>t_\<AA> = (\<lambda> (in\<^sub>P\<^sub>l\<^sub>a\<^sub>n\<^sub>e\<^sub>t (Planet)) \<Rightarrow> \<lfloor>Planet\<rfloor>
-    | (in\<^sub>G\<^sub>a\<^sub>l\<^sub>a\<^sub>x\<^sub>y ((mkoid\<^sub>G\<^sub>a\<^sub>l\<^sub>a\<^sub>x\<^sub>y ((mk\<^sub>G\<^sub>a\<^sub>l\<^sub>a\<^sub>x\<^sub>y_\<^sub>P\<^sub>l\<^sub>a\<^sub>n\<^sub>e\<^sub>t (Planet))) (_) (_) (_)))) \<Rightarrow> \<lfloor>Planet\<rfloor>
-    | (in\<^sub>O\<^sub>c\<^sub>l\<^sub>A\<^sub>n\<^sub>y ((mkoid\<^sub>O\<^sub>c\<^sub>l\<^sub>A\<^sub>n\<^sub>y ((mk\<^sub>O\<^sub>c\<^sub>l\<^sub>A\<^sub>n\<^sub>y_\<^sub>P\<^sub>l\<^sub>a\<^sub>n\<^sub>e\<^sub>t (Planet)))))) \<Rightarrow> \<lfloor>Planet\<rfloor>
-    | (in\<^sub>P\<^sub>e\<^sub>r\<^sub>s\<^sub>o\<^sub>n (Person)) \<Rightarrow> \<lfloor>(mkoid\<^sub>P\<^sub>l\<^sub>a\<^sub>n\<^sub>e\<^sub>t ((mk\<^sub>P\<^sub>l\<^sub>a\<^sub>n\<^sub>e\<^sub>t_\<^sub>P\<^sub>e\<^sub>r\<^sub>s\<^sub>o\<^sub>n (Person))) (None) (None))\<rfloor>
+    | (in\<^sub>G\<^sub>a\<^sub>l\<^sub>a\<^sub>x\<^sub>y ((mk\<^sub>G\<^sub>a\<^sub>l\<^sub>a\<^sub>x\<^sub>y ((mk\<E>\<X>\<T>\<^sub>G\<^sub>a\<^sub>l\<^sub>a\<^sub>x\<^sub>y_\<^sub>P\<^sub>l\<^sub>a\<^sub>n\<^sub>e\<^sub>t (Planet))) (_) (_) (_)))) \<Rightarrow> \<lfloor>Planet\<rfloor>
+    | (in\<^sub>O\<^sub>c\<^sub>l\<^sub>A\<^sub>n\<^sub>y ((mk\<^sub>O\<^sub>c\<^sub>l\<^sub>A\<^sub>n\<^sub>y ((mk\<E>\<X>\<T>\<^sub>O\<^sub>c\<^sub>l\<^sub>A\<^sub>n\<^sub>y_\<^sub>P\<^sub>l\<^sub>a\<^sub>n\<^sub>e\<^sub>t (Planet)))))) \<Rightarrow> \<lfloor>Planet\<rfloor>
+    | (in\<^sub>P\<^sub>e\<^sub>r\<^sub>s\<^sub>o\<^sub>n (Person)) \<Rightarrow> \<lfloor>(mk\<^sub>P\<^sub>l\<^sub>a\<^sub>n\<^sub>e\<^sub>t ((mk\<E>\<X>\<T>\<^sub>P\<^sub>l\<^sub>a\<^sub>n\<^sub>e\<^sub>t_\<^sub>P\<^sub>e\<^sub>r\<^sub>s\<^sub>o\<^sub>n (Person))) (None) (None))\<rfloor>
     | _ \<Rightarrow> None)"
 definition "OclAsType\<^sub>G\<^sub>a\<^sub>l\<^sub>a\<^sub>x\<^sub>y_\<AA> = (\<lambda> (in\<^sub>G\<^sub>a\<^sub>l\<^sub>a\<^sub>x\<^sub>y (Galaxy)) \<Rightarrow> \<lfloor>Galaxy\<rfloor>
-    | (in\<^sub>O\<^sub>c\<^sub>l\<^sub>A\<^sub>n\<^sub>y ((mkoid\<^sub>O\<^sub>c\<^sub>l\<^sub>A\<^sub>n\<^sub>y ((mk\<^sub>O\<^sub>c\<^sub>l\<^sub>A\<^sub>n\<^sub>y_\<^sub>G\<^sub>a\<^sub>l\<^sub>a\<^sub>x\<^sub>y (Galaxy)))))) \<Rightarrow> \<lfloor>Galaxy\<rfloor>
-    | (in\<^sub>P\<^sub>e\<^sub>r\<^sub>s\<^sub>o\<^sub>n (Person)) \<Rightarrow> \<lfloor>(mkoid\<^sub>G\<^sub>a\<^sub>l\<^sub>a\<^sub>x\<^sub>y ((mk\<^sub>G\<^sub>a\<^sub>l\<^sub>a\<^sub>x\<^sub>y_\<^sub>P\<^sub>e\<^sub>r\<^sub>s\<^sub>o\<^sub>n (Person))) (None) (None) (None))\<rfloor>
-    | (in\<^sub>P\<^sub>l\<^sub>a\<^sub>n\<^sub>e\<^sub>t (Planet)) \<Rightarrow> \<lfloor>(mkoid\<^sub>G\<^sub>a\<^sub>l\<^sub>a\<^sub>x\<^sub>y ((mk\<^sub>G\<^sub>a\<^sub>l\<^sub>a\<^sub>x\<^sub>y_\<^sub>P\<^sub>l\<^sub>a\<^sub>n\<^sub>e\<^sub>t (Planet))) (None) (None) (None))\<rfloor>
+    | (in\<^sub>O\<^sub>c\<^sub>l\<^sub>A\<^sub>n\<^sub>y ((mk\<^sub>O\<^sub>c\<^sub>l\<^sub>A\<^sub>n\<^sub>y ((mk\<E>\<X>\<T>\<^sub>O\<^sub>c\<^sub>l\<^sub>A\<^sub>n\<^sub>y_\<^sub>G\<^sub>a\<^sub>l\<^sub>a\<^sub>x\<^sub>y (Galaxy)))))) \<Rightarrow> \<lfloor>Galaxy\<rfloor>
+    | (in\<^sub>P\<^sub>e\<^sub>r\<^sub>s\<^sub>o\<^sub>n (Person)) \<Rightarrow> \<lfloor>(mk\<^sub>G\<^sub>a\<^sub>l\<^sub>a\<^sub>x\<^sub>y ((mk\<E>\<X>\<T>\<^sub>G\<^sub>a\<^sub>l\<^sub>a\<^sub>x\<^sub>y_\<^sub>P\<^sub>e\<^sub>r\<^sub>s\<^sub>o\<^sub>n (Person))) (None) (None) (None))\<rfloor>
+    | (in\<^sub>P\<^sub>l\<^sub>a\<^sub>n\<^sub>e\<^sub>t (Planet)) \<Rightarrow> \<lfloor>(mk\<^sub>G\<^sub>a\<^sub>l\<^sub>a\<^sub>x\<^sub>y ((mk\<E>\<X>\<T>\<^sub>G\<^sub>a\<^sub>l\<^sub>a\<^sub>x\<^sub>y_\<^sub>P\<^sub>l\<^sub>a\<^sub>n\<^sub>e\<^sub>t (Planet))) (None) (None) (None))\<rfloor>
     | _ \<Rightarrow> None)"
 definition "OclAsType\<^sub>O\<^sub>c\<^sub>l\<^sub>A\<^sub>n\<^sub>y_\<AA> = Some o (\<lambda> (in\<^sub>O\<^sub>c\<^sub>l\<^sub>A\<^sub>n\<^sub>y (OclAny)) \<Rightarrow> OclAny
-    | (in\<^sub>P\<^sub>e\<^sub>r\<^sub>s\<^sub>o\<^sub>n (Person)) \<Rightarrow> (mkoid\<^sub>O\<^sub>c\<^sub>l\<^sub>A\<^sub>n\<^sub>y ((mk\<^sub>O\<^sub>c\<^sub>l\<^sub>A\<^sub>n\<^sub>y_\<^sub>P\<^sub>e\<^sub>r\<^sub>s\<^sub>o\<^sub>n (Person))))
-    | (in\<^sub>P\<^sub>l\<^sub>a\<^sub>n\<^sub>e\<^sub>t (Planet)) \<Rightarrow> (mkoid\<^sub>O\<^sub>c\<^sub>l\<^sub>A\<^sub>n\<^sub>y ((mk\<^sub>O\<^sub>c\<^sub>l\<^sub>A\<^sub>n\<^sub>y_\<^sub>P\<^sub>l\<^sub>a\<^sub>n\<^sub>e\<^sub>t (Planet))))
-    | (in\<^sub>G\<^sub>a\<^sub>l\<^sub>a\<^sub>x\<^sub>y (Galaxy)) \<Rightarrow> (mkoid\<^sub>O\<^sub>c\<^sub>l\<^sub>A\<^sub>n\<^sub>y ((mk\<^sub>O\<^sub>c\<^sub>l\<^sub>A\<^sub>n\<^sub>y_\<^sub>G\<^sub>a\<^sub>l\<^sub>a\<^sub>x\<^sub>y (Galaxy)))))"
+    | (in\<^sub>P\<^sub>e\<^sub>r\<^sub>s\<^sub>o\<^sub>n (Person)) \<Rightarrow> (mk\<^sub>O\<^sub>c\<^sub>l\<^sub>A\<^sub>n\<^sub>y ((mk\<E>\<X>\<T>\<^sub>O\<^sub>c\<^sub>l\<^sub>A\<^sub>n\<^sub>y_\<^sub>P\<^sub>e\<^sub>r\<^sub>s\<^sub>o\<^sub>n (Person))))
+    | (in\<^sub>P\<^sub>l\<^sub>a\<^sub>n\<^sub>e\<^sub>t (Planet)) \<Rightarrow> (mk\<^sub>O\<^sub>c\<^sub>l\<^sub>A\<^sub>n\<^sub>y ((mk\<E>\<X>\<T>\<^sub>O\<^sub>c\<^sub>l\<^sub>A\<^sub>n\<^sub>y_\<^sub>P\<^sub>l\<^sub>a\<^sub>n\<^sub>e\<^sub>t (Planet))))
+    | (in\<^sub>G\<^sub>a\<^sub>l\<^sub>a\<^sub>x\<^sub>y (Galaxy)) \<Rightarrow> (mk\<^sub>O\<^sub>c\<^sub>l\<^sub>A\<^sub>n\<^sub>y ((mk\<E>\<X>\<T>\<^sub>O\<^sub>c\<^sub>l\<^sub>A\<^sub>n\<^sub>y_\<^sub>G\<^sub>a\<^sub>l\<^sub>a\<^sub>x\<^sub>y (Galaxy)))))"
 
 (* 34 ************************************ 77 + 1 *)
 lemmas[simp,code_unfold] = OclAsType\<^sub>P\<^sub>e\<^sub>r\<^sub>s\<^sub>o\<^sub>n_Person
@@ -634,32 +634,32 @@ lemma up\<^sub>P\<^sub>l\<^sub>a\<^sub>n\<^sub>e\<^sub>t_down\<^sub>P\<^sub>e\<^
 assumes isdef: "\<tau> \<Turnstile> (\<delta> (X))"
 shows "\<tau> \<Turnstile> (((X::Person) .oclAsType(Planet)) .oclAsType(Person)) \<triangleq> X"
   using isdef
-by(auto simp: OclAsType\<^sub>P\<^sub>l\<^sub>a\<^sub>n\<^sub>e\<^sub>t_Person OclAsType\<^sub>P\<^sub>e\<^sub>r\<^sub>s\<^sub>o\<^sub>n_Planet foundation22 foundation16 null_option_def bot_option_def split: type\<^sub>P\<^sub>e\<^sub>r\<^sub>s\<^sub>o\<^sub>n.split typeoid\<^sub>P\<^sub>e\<^sub>r\<^sub>s\<^sub>o\<^sub>n.split) 
+by(auto simp: OclAsType\<^sub>P\<^sub>l\<^sub>a\<^sub>n\<^sub>e\<^sub>t_Person OclAsType\<^sub>P\<^sub>e\<^sub>r\<^sub>s\<^sub>o\<^sub>n_Planet foundation22 foundation16 null_option_def bot_option_def split: ty\<E>\<X>\<T>\<^sub>P\<^sub>e\<^sub>r\<^sub>s\<^sub>o\<^sub>n.split ty\<^sub>P\<^sub>e\<^sub>r\<^sub>s\<^sub>o\<^sub>n.split) 
 lemma up\<^sub>G\<^sub>a\<^sub>l\<^sub>a\<^sub>x\<^sub>y_down\<^sub>P\<^sub>e\<^sub>r\<^sub>s\<^sub>o\<^sub>n_cast0 : 
 assumes isdef: "\<tau> \<Turnstile> (\<delta> (X))"
 shows "\<tau> \<Turnstile> (((X::Person) .oclAsType(Galaxy)) .oclAsType(Person)) \<triangleq> X"
   using isdef
-by(auto simp: OclAsType\<^sub>G\<^sub>a\<^sub>l\<^sub>a\<^sub>x\<^sub>y_Person OclAsType\<^sub>P\<^sub>e\<^sub>r\<^sub>s\<^sub>o\<^sub>n_Galaxy foundation22 foundation16 null_option_def bot_option_def split: type\<^sub>P\<^sub>e\<^sub>r\<^sub>s\<^sub>o\<^sub>n.split typeoid\<^sub>P\<^sub>e\<^sub>r\<^sub>s\<^sub>o\<^sub>n.split) 
+by(auto simp: OclAsType\<^sub>G\<^sub>a\<^sub>l\<^sub>a\<^sub>x\<^sub>y_Person OclAsType\<^sub>P\<^sub>e\<^sub>r\<^sub>s\<^sub>o\<^sub>n_Galaxy foundation22 foundation16 null_option_def bot_option_def split: ty\<E>\<X>\<T>\<^sub>P\<^sub>e\<^sub>r\<^sub>s\<^sub>o\<^sub>n.split ty\<^sub>P\<^sub>e\<^sub>r\<^sub>s\<^sub>o\<^sub>n.split) 
 lemma up\<^sub>O\<^sub>c\<^sub>l\<^sub>A\<^sub>n\<^sub>y_down\<^sub>P\<^sub>e\<^sub>r\<^sub>s\<^sub>o\<^sub>n_cast0 : 
 assumes isdef: "\<tau> \<Turnstile> (\<delta> (X))"
 shows "\<tau> \<Turnstile> (((X::Person) .oclAsType(OclAny)) .oclAsType(Person)) \<triangleq> X"
   using isdef
-by(auto simp: OclAsType\<^sub>O\<^sub>c\<^sub>l\<^sub>A\<^sub>n\<^sub>y_Person OclAsType\<^sub>P\<^sub>e\<^sub>r\<^sub>s\<^sub>o\<^sub>n_OclAny foundation22 foundation16 null_option_def bot_option_def split: type\<^sub>P\<^sub>e\<^sub>r\<^sub>s\<^sub>o\<^sub>n.split typeoid\<^sub>P\<^sub>e\<^sub>r\<^sub>s\<^sub>o\<^sub>n.split) 
+by(auto simp: OclAsType\<^sub>O\<^sub>c\<^sub>l\<^sub>A\<^sub>n\<^sub>y_Person OclAsType\<^sub>P\<^sub>e\<^sub>r\<^sub>s\<^sub>o\<^sub>n_OclAny foundation22 foundation16 null_option_def bot_option_def split: ty\<E>\<X>\<T>\<^sub>P\<^sub>e\<^sub>r\<^sub>s\<^sub>o\<^sub>n.split ty\<^sub>P\<^sub>e\<^sub>r\<^sub>s\<^sub>o\<^sub>n.split) 
 lemma up\<^sub>G\<^sub>a\<^sub>l\<^sub>a\<^sub>x\<^sub>y_down\<^sub>P\<^sub>l\<^sub>a\<^sub>n\<^sub>e\<^sub>t_cast0 : 
 assumes isdef: "\<tau> \<Turnstile> (\<delta> (X))"
 shows "\<tau> \<Turnstile> (((X::Planet) .oclAsType(Galaxy)) .oclAsType(Planet)) \<triangleq> X"
   using isdef
-by(auto simp: OclAsType\<^sub>G\<^sub>a\<^sub>l\<^sub>a\<^sub>x\<^sub>y_Planet OclAsType\<^sub>P\<^sub>l\<^sub>a\<^sub>n\<^sub>e\<^sub>t_Galaxy foundation22 foundation16 null_option_def bot_option_def split: type\<^sub>P\<^sub>l\<^sub>a\<^sub>n\<^sub>e\<^sub>t.split typeoid\<^sub>P\<^sub>l\<^sub>a\<^sub>n\<^sub>e\<^sub>t.split) 
+by(auto simp: OclAsType\<^sub>G\<^sub>a\<^sub>l\<^sub>a\<^sub>x\<^sub>y_Planet OclAsType\<^sub>P\<^sub>l\<^sub>a\<^sub>n\<^sub>e\<^sub>t_Galaxy foundation22 foundation16 null_option_def bot_option_def split: ty\<E>\<X>\<T>\<^sub>P\<^sub>l\<^sub>a\<^sub>n\<^sub>e\<^sub>t.split ty\<^sub>P\<^sub>l\<^sub>a\<^sub>n\<^sub>e\<^sub>t.split) 
 lemma up\<^sub>O\<^sub>c\<^sub>l\<^sub>A\<^sub>n\<^sub>y_down\<^sub>P\<^sub>l\<^sub>a\<^sub>n\<^sub>e\<^sub>t_cast0 : 
 assumes isdef: "\<tau> \<Turnstile> (\<delta> (X))"
 shows "\<tau> \<Turnstile> (((X::Planet) .oclAsType(OclAny)) .oclAsType(Planet)) \<triangleq> X"
   using isdef
-by(auto simp: OclAsType\<^sub>O\<^sub>c\<^sub>l\<^sub>A\<^sub>n\<^sub>y_Planet OclAsType\<^sub>P\<^sub>l\<^sub>a\<^sub>n\<^sub>e\<^sub>t_OclAny foundation22 foundation16 null_option_def bot_option_def split: type\<^sub>P\<^sub>l\<^sub>a\<^sub>n\<^sub>e\<^sub>t.split typeoid\<^sub>P\<^sub>l\<^sub>a\<^sub>n\<^sub>e\<^sub>t.split) 
+by(auto simp: OclAsType\<^sub>O\<^sub>c\<^sub>l\<^sub>A\<^sub>n\<^sub>y_Planet OclAsType\<^sub>P\<^sub>l\<^sub>a\<^sub>n\<^sub>e\<^sub>t_OclAny foundation22 foundation16 null_option_def bot_option_def split: ty\<E>\<X>\<T>\<^sub>P\<^sub>l\<^sub>a\<^sub>n\<^sub>e\<^sub>t.split ty\<^sub>P\<^sub>l\<^sub>a\<^sub>n\<^sub>e\<^sub>t.split) 
 lemma up\<^sub>O\<^sub>c\<^sub>l\<^sub>A\<^sub>n\<^sub>y_down\<^sub>G\<^sub>a\<^sub>l\<^sub>a\<^sub>x\<^sub>y_cast0 : 
 assumes isdef: "\<tau> \<Turnstile> (\<delta> (X))"
 shows "\<tau> \<Turnstile> (((X::Galaxy) .oclAsType(OclAny)) .oclAsType(Galaxy)) \<triangleq> X"
   using isdef
-by(auto simp: OclAsType\<^sub>O\<^sub>c\<^sub>l\<^sub>A\<^sub>n\<^sub>y_Galaxy OclAsType\<^sub>G\<^sub>a\<^sub>l\<^sub>a\<^sub>x\<^sub>y_OclAny foundation22 foundation16 null_option_def bot_option_def split: type\<^sub>G\<^sub>a\<^sub>l\<^sub>a\<^sub>x\<^sub>y.split typeoid\<^sub>G\<^sub>a\<^sub>l\<^sub>a\<^sub>x\<^sub>y.split) 
+by(auto simp: OclAsType\<^sub>O\<^sub>c\<^sub>l\<^sub>A\<^sub>n\<^sub>y_Galaxy OclAsType\<^sub>G\<^sub>a\<^sub>l\<^sub>a\<^sub>x\<^sub>y_OclAny foundation22 foundation16 null_option_def bot_option_def split: ty\<E>\<X>\<T>\<^sub>G\<^sub>a\<^sub>l\<^sub>a\<^sub>x\<^sub>y.split ty\<^sub>G\<^sub>a\<^sub>l\<^sub>a\<^sub>x\<^sub>y.split) 
 
 (* 45 ************************************ 192 + 6 *)
 lemma up\<^sub>P\<^sub>l\<^sub>a\<^sub>n\<^sub>e\<^sub>t_down\<^sub>P\<^sub>e\<^sub>r\<^sub>s\<^sub>o\<^sub>n_cast : 
@@ -758,41 +758,41 @@ consts OclIsTypeOf\<^sub>O\<^sub>c\<^sub>l\<^sub>A\<^sub>n\<^sub>y :: "'\<alpha>
 (* 50 ************************************ 210 + 16 *)
 defs(overloaded) OclIsTypeOf\<^sub>P\<^sub>e\<^sub>r\<^sub>s\<^sub>o\<^sub>n_Person : "(x::Person) .oclIsTypeOf(Person) \<equiv> (\<lambda>\<tau>. (case (x (\<tau>)) of \<bottom> \<Rightarrow> (invalid (\<tau>))
     | \<lfloor>\<bottom>\<rfloor> \<Rightarrow> (true (\<tau>))
-    | \<lfloor>\<lfloor>(mkoid\<^sub>P\<^sub>e\<^sub>r\<^sub>s\<^sub>o\<^sub>n ((mk\<^sub>P\<^sub>e\<^sub>r\<^sub>s\<^sub>o\<^sub>n (_) (_) (_) (_) (_) (_))) (_) (_))\<rfloor>\<rfloor> \<Rightarrow> (true (\<tau>))))"
+    | \<lfloor>\<lfloor>(mk\<^sub>P\<^sub>e\<^sub>r\<^sub>s\<^sub>o\<^sub>n ((mk\<E>\<X>\<T>\<^sub>P\<^sub>e\<^sub>r\<^sub>s\<^sub>o\<^sub>n (_) (_) (_) (_) (_) (_))) (_) (_))\<rfloor>\<rfloor> \<Rightarrow> (true (\<tau>))))"
 defs(overloaded) OclIsTypeOf\<^sub>P\<^sub>e\<^sub>r\<^sub>s\<^sub>o\<^sub>n_Planet : "(x::Planet) .oclIsTypeOf(Person) \<equiv> (\<lambda>\<tau>. (case (x (\<tau>)) of \<bottom> \<Rightarrow> (invalid (\<tau>))
     | \<lfloor>\<bottom>\<rfloor> \<Rightarrow> (true (\<tau>))
-    | \<lfloor>\<lfloor>(mkoid\<^sub>P\<^sub>l\<^sub>a\<^sub>n\<^sub>e\<^sub>t ((mk\<^sub>P\<^sub>l\<^sub>a\<^sub>n\<^sub>e\<^sub>t_\<^sub>P\<^sub>e\<^sub>r\<^sub>s\<^sub>o\<^sub>n (_))) (_) (_))\<rfloor>\<rfloor> \<Rightarrow> (true (\<tau>))
+    | \<lfloor>\<lfloor>(mk\<^sub>P\<^sub>l\<^sub>a\<^sub>n\<^sub>e\<^sub>t ((mk\<E>\<X>\<T>\<^sub>P\<^sub>l\<^sub>a\<^sub>n\<^sub>e\<^sub>t_\<^sub>P\<^sub>e\<^sub>r\<^sub>s\<^sub>o\<^sub>n (_))) (_) (_))\<rfloor>\<rfloor> \<Rightarrow> (true (\<tau>))
     | _ \<Rightarrow> (false (\<tau>))))"
 defs(overloaded) OclIsTypeOf\<^sub>P\<^sub>e\<^sub>r\<^sub>s\<^sub>o\<^sub>n_Galaxy : "(x::Galaxy) .oclIsTypeOf(Person) \<equiv> (\<lambda>\<tau>. (case (x (\<tau>)) of \<bottom> \<Rightarrow> (invalid (\<tau>))
     | \<lfloor>\<bottom>\<rfloor> \<Rightarrow> (true (\<tau>))
-    | \<lfloor>\<lfloor>(mkoid\<^sub>G\<^sub>a\<^sub>l\<^sub>a\<^sub>x\<^sub>y ((mk\<^sub>G\<^sub>a\<^sub>l\<^sub>a\<^sub>x\<^sub>y_\<^sub>P\<^sub>e\<^sub>r\<^sub>s\<^sub>o\<^sub>n (_))) (_) (_) (_))\<rfloor>\<rfloor> \<Rightarrow> (true (\<tau>))
+    | \<lfloor>\<lfloor>(mk\<^sub>G\<^sub>a\<^sub>l\<^sub>a\<^sub>x\<^sub>y ((mk\<E>\<X>\<T>\<^sub>G\<^sub>a\<^sub>l\<^sub>a\<^sub>x\<^sub>y_\<^sub>P\<^sub>e\<^sub>r\<^sub>s\<^sub>o\<^sub>n (_))) (_) (_) (_))\<rfloor>\<rfloor> \<Rightarrow> (true (\<tau>))
     | _ \<Rightarrow> (false (\<tau>))))"
 defs(overloaded) OclIsTypeOf\<^sub>P\<^sub>e\<^sub>r\<^sub>s\<^sub>o\<^sub>n_OclAny : "(x::OclAny) .oclIsTypeOf(Person) \<equiv> (\<lambda>\<tau>. (case (x (\<tau>)) of \<bottom> \<Rightarrow> (invalid (\<tau>))
     | \<lfloor>\<bottom>\<rfloor> \<Rightarrow> (true (\<tau>))
-    | \<lfloor>\<lfloor>(mkoid\<^sub>O\<^sub>c\<^sub>l\<^sub>A\<^sub>n\<^sub>y ((mk\<^sub>O\<^sub>c\<^sub>l\<^sub>A\<^sub>n\<^sub>y_\<^sub>P\<^sub>e\<^sub>r\<^sub>s\<^sub>o\<^sub>n (_))))\<rfloor>\<rfloor> \<Rightarrow> (true (\<tau>))
+    | \<lfloor>\<lfloor>(mk\<^sub>O\<^sub>c\<^sub>l\<^sub>A\<^sub>n\<^sub>y ((mk\<E>\<X>\<T>\<^sub>O\<^sub>c\<^sub>l\<^sub>A\<^sub>n\<^sub>y_\<^sub>P\<^sub>e\<^sub>r\<^sub>s\<^sub>o\<^sub>n (_))))\<rfloor>\<rfloor> \<Rightarrow> (true (\<tau>))
     | _ \<Rightarrow> (false (\<tau>))))"
 defs(overloaded) OclIsTypeOf\<^sub>P\<^sub>l\<^sub>a\<^sub>n\<^sub>e\<^sub>t_Planet : "(x::Planet) .oclIsTypeOf(Planet) \<equiv> (\<lambda>\<tau>. (case (x (\<tau>)) of \<bottom> \<Rightarrow> (invalid (\<tau>))
     | \<lfloor>\<bottom>\<rfloor> \<Rightarrow> (true (\<tau>))
-    | \<lfloor>\<lfloor>(mkoid\<^sub>P\<^sub>l\<^sub>a\<^sub>n\<^sub>e\<^sub>t ((mk\<^sub>P\<^sub>l\<^sub>a\<^sub>n\<^sub>e\<^sub>t (_) (_) (_) (_))) (_) (_))\<rfloor>\<rfloor> \<Rightarrow> (true (\<tau>))
+    | \<lfloor>\<lfloor>(mk\<^sub>P\<^sub>l\<^sub>a\<^sub>n\<^sub>e\<^sub>t ((mk\<E>\<X>\<T>\<^sub>P\<^sub>l\<^sub>a\<^sub>n\<^sub>e\<^sub>t (_) (_) (_) (_))) (_) (_))\<rfloor>\<rfloor> \<Rightarrow> (true (\<tau>))
     | _ \<Rightarrow> (false (\<tau>))))"
 defs(overloaded) OclIsTypeOf\<^sub>P\<^sub>l\<^sub>a\<^sub>n\<^sub>e\<^sub>t_Galaxy : "(x::Galaxy) .oclIsTypeOf(Planet) \<equiv> (\<lambda>\<tau>. (case (x (\<tau>)) of \<bottom> \<Rightarrow> (invalid (\<tau>))
     | \<lfloor>\<bottom>\<rfloor> \<Rightarrow> (true (\<tau>))
-    | \<lfloor>\<lfloor>(mkoid\<^sub>G\<^sub>a\<^sub>l\<^sub>a\<^sub>x\<^sub>y ((mk\<^sub>G\<^sub>a\<^sub>l\<^sub>a\<^sub>x\<^sub>y_\<^sub>P\<^sub>l\<^sub>a\<^sub>n\<^sub>e\<^sub>t (_))) (_) (_) (_))\<rfloor>\<rfloor> \<Rightarrow> (true (\<tau>))
+    | \<lfloor>\<lfloor>(mk\<^sub>G\<^sub>a\<^sub>l\<^sub>a\<^sub>x\<^sub>y ((mk\<E>\<X>\<T>\<^sub>G\<^sub>a\<^sub>l\<^sub>a\<^sub>x\<^sub>y_\<^sub>P\<^sub>l\<^sub>a\<^sub>n\<^sub>e\<^sub>t (_))) (_) (_) (_))\<rfloor>\<rfloor> \<Rightarrow> (true (\<tau>))
     | _ \<Rightarrow> (false (\<tau>))))"
 defs(overloaded) OclIsTypeOf\<^sub>P\<^sub>l\<^sub>a\<^sub>n\<^sub>e\<^sub>t_OclAny : "(x::OclAny) .oclIsTypeOf(Planet) \<equiv> (\<lambda>\<tau>. (case (x (\<tau>)) of \<bottom> \<Rightarrow> (invalid (\<tau>))
     | \<lfloor>\<bottom>\<rfloor> \<Rightarrow> (true (\<tau>))
-    | \<lfloor>\<lfloor>(mkoid\<^sub>O\<^sub>c\<^sub>l\<^sub>A\<^sub>n\<^sub>y ((mk\<^sub>O\<^sub>c\<^sub>l\<^sub>A\<^sub>n\<^sub>y_\<^sub>P\<^sub>l\<^sub>a\<^sub>n\<^sub>e\<^sub>t (_))))\<rfloor>\<rfloor> \<Rightarrow> (true (\<tau>))
+    | \<lfloor>\<lfloor>(mk\<^sub>O\<^sub>c\<^sub>l\<^sub>A\<^sub>n\<^sub>y ((mk\<E>\<X>\<T>\<^sub>O\<^sub>c\<^sub>l\<^sub>A\<^sub>n\<^sub>y_\<^sub>P\<^sub>l\<^sub>a\<^sub>n\<^sub>e\<^sub>t (_))))\<rfloor>\<rfloor> \<Rightarrow> (true (\<tau>))
     | _ \<Rightarrow> (false (\<tau>))))"
 defs(overloaded) OclIsTypeOf\<^sub>P\<^sub>l\<^sub>a\<^sub>n\<^sub>e\<^sub>t_Person : "(x::Person) .oclIsTypeOf(Planet) \<equiv> (\<lambda>\<tau>. (case (x (\<tau>)) of \<bottom> \<Rightarrow> (invalid (\<tau>))
     | \<lfloor>\<bottom>\<rfloor> \<Rightarrow> (true (\<tau>))
     | _ \<Rightarrow> (false (\<tau>))))"
 defs(overloaded) OclIsTypeOf\<^sub>G\<^sub>a\<^sub>l\<^sub>a\<^sub>x\<^sub>y_Galaxy : "(x::Galaxy) .oclIsTypeOf(Galaxy) \<equiv> (\<lambda>\<tau>. (case (x (\<tau>)) of \<bottom> \<Rightarrow> (invalid (\<tau>))
     | \<lfloor>\<bottom>\<rfloor> \<Rightarrow> (true (\<tau>))
-    | \<lfloor>\<lfloor>(mkoid\<^sub>G\<^sub>a\<^sub>l\<^sub>a\<^sub>x\<^sub>y ((mk\<^sub>G\<^sub>a\<^sub>l\<^sub>a\<^sub>x\<^sub>y (_))) (_) (_) (_))\<rfloor>\<rfloor> \<Rightarrow> (true (\<tau>))
+    | \<lfloor>\<lfloor>(mk\<^sub>G\<^sub>a\<^sub>l\<^sub>a\<^sub>x\<^sub>y ((mk\<E>\<X>\<T>\<^sub>G\<^sub>a\<^sub>l\<^sub>a\<^sub>x\<^sub>y (_))) (_) (_) (_))\<rfloor>\<rfloor> \<Rightarrow> (true (\<tau>))
     | _ \<Rightarrow> (false (\<tau>))))"
 defs(overloaded) OclIsTypeOf\<^sub>G\<^sub>a\<^sub>l\<^sub>a\<^sub>x\<^sub>y_OclAny : "(x::OclAny) .oclIsTypeOf(Galaxy) \<equiv> (\<lambda>\<tau>. (case (x (\<tau>)) of \<bottom> \<Rightarrow> (invalid (\<tau>))
     | \<lfloor>\<bottom>\<rfloor> \<Rightarrow> (true (\<tau>))
-    | \<lfloor>\<lfloor>(mkoid\<^sub>O\<^sub>c\<^sub>l\<^sub>A\<^sub>n\<^sub>y ((mk\<^sub>O\<^sub>c\<^sub>l\<^sub>A\<^sub>n\<^sub>y_\<^sub>G\<^sub>a\<^sub>l\<^sub>a\<^sub>x\<^sub>y (_))))\<rfloor>\<rfloor> \<Rightarrow> (true (\<tau>))
+    | \<lfloor>\<lfloor>(mk\<^sub>O\<^sub>c\<^sub>l\<^sub>A\<^sub>n\<^sub>y ((mk\<E>\<X>\<T>\<^sub>O\<^sub>c\<^sub>l\<^sub>A\<^sub>n\<^sub>y_\<^sub>G\<^sub>a\<^sub>l\<^sub>a\<^sub>x\<^sub>y (_))))\<rfloor>\<rfloor> \<Rightarrow> (true (\<tau>))
     | _ \<Rightarrow> (false (\<tau>))))"
 defs(overloaded) OclIsTypeOf\<^sub>G\<^sub>a\<^sub>l\<^sub>a\<^sub>x\<^sub>y_Person : "(x::Person) .oclIsTypeOf(Galaxy) \<equiv> (\<lambda>\<tau>. (case (x (\<tau>)) of \<bottom> \<Rightarrow> (invalid (\<tau>))
     | \<lfloor>\<bottom>\<rfloor> \<Rightarrow> (true (\<tau>))
@@ -802,7 +802,7 @@ defs(overloaded) OclIsTypeOf\<^sub>G\<^sub>a\<^sub>l\<^sub>a\<^sub>x\<^sub>y_Pla
     | _ \<Rightarrow> (false (\<tau>))))"
 defs(overloaded) OclIsTypeOf\<^sub>O\<^sub>c\<^sub>l\<^sub>A\<^sub>n\<^sub>y_OclAny : "(x::OclAny) .oclIsTypeOf(OclAny) \<equiv> (\<lambda>\<tau>. (case (x (\<tau>)) of \<bottom> \<Rightarrow> (invalid (\<tau>))
     | \<lfloor>\<bottom>\<rfloor> \<Rightarrow> (true (\<tau>))
-    | \<lfloor>\<lfloor>(mkoid\<^sub>O\<^sub>c\<^sub>l\<^sub>A\<^sub>n\<^sub>y ((mk\<^sub>O\<^sub>c\<^sub>l\<^sub>A\<^sub>n\<^sub>y (_))))\<rfloor>\<rfloor> \<Rightarrow> (true (\<tau>))
+    | \<lfloor>\<lfloor>(mk\<^sub>O\<^sub>c\<^sub>l\<^sub>A\<^sub>n\<^sub>y ((mk\<E>\<X>\<T>\<^sub>O\<^sub>c\<^sub>l\<^sub>A\<^sub>n\<^sub>y (_))))\<rfloor>\<rfloor> \<Rightarrow> (true (\<tau>))
     | _ \<Rightarrow> (false (\<tau>))))"
 defs(overloaded) OclIsTypeOf\<^sub>O\<^sub>c\<^sub>l\<^sub>A\<^sub>n\<^sub>y_Person : "(x::Person) .oclIsTypeOf(OclAny) \<equiv> (\<lambda>\<tau>. (case (x (\<tau>)) of \<bottom> \<Rightarrow> (invalid (\<tau>))
     | \<lfloor>\<bottom>\<rfloor> \<Rightarrow> (true (\<tau>))
@@ -1148,82 +1148,82 @@ lemma OclIsTypeOf\<^sub>P\<^sub>e\<^sub>r\<^sub>s\<^sub>o\<^sub>n_Person_defined
 assumes isdef: "\<tau> \<Turnstile> (\<upsilon> (X))"
 shows "\<tau> \<Turnstile> (\<delta> ((X::Person) .oclIsTypeOf(Person)))"
   apply(insert isdef[simplified foundation18'], simp only: OclValid_def, subst cp_defined)
-by(auto simp: cp_defined[symmetric ] bot_option_def OclIsTypeOf\<^sub>P\<^sub>e\<^sub>r\<^sub>s\<^sub>o\<^sub>n_Person split: option.split type\<^sub>P\<^sub>e\<^sub>r\<^sub>s\<^sub>o\<^sub>n.split typeoid\<^sub>P\<^sub>e\<^sub>r\<^sub>s\<^sub>o\<^sub>n.split) 
+by(auto simp: cp_defined[symmetric ] bot_option_def OclIsTypeOf\<^sub>P\<^sub>e\<^sub>r\<^sub>s\<^sub>o\<^sub>n_Person split: option.split ty\<E>\<X>\<T>\<^sub>P\<^sub>e\<^sub>r\<^sub>s\<^sub>o\<^sub>n.split ty\<^sub>P\<^sub>e\<^sub>r\<^sub>s\<^sub>o\<^sub>n.split) 
 lemma OclIsTypeOf\<^sub>P\<^sub>e\<^sub>r\<^sub>s\<^sub>o\<^sub>n_Planet_defined : 
 assumes isdef: "\<tau> \<Turnstile> (\<upsilon> (X))"
 shows "\<tau> \<Turnstile> (\<delta> ((X::Planet) .oclIsTypeOf(Person)))"
   apply(insert isdef[simplified foundation18'], simp only: OclValid_def, subst cp_defined)
-by(auto simp: cp_defined[symmetric ] bot_option_def OclIsTypeOf\<^sub>P\<^sub>e\<^sub>r\<^sub>s\<^sub>o\<^sub>n_Planet split: option.split type\<^sub>P\<^sub>l\<^sub>a\<^sub>n\<^sub>e\<^sub>t.split typeoid\<^sub>P\<^sub>l\<^sub>a\<^sub>n\<^sub>e\<^sub>t.split) 
+by(auto simp: cp_defined[symmetric ] bot_option_def OclIsTypeOf\<^sub>P\<^sub>e\<^sub>r\<^sub>s\<^sub>o\<^sub>n_Planet split: option.split ty\<E>\<X>\<T>\<^sub>P\<^sub>l\<^sub>a\<^sub>n\<^sub>e\<^sub>t.split ty\<^sub>P\<^sub>l\<^sub>a\<^sub>n\<^sub>e\<^sub>t.split) 
 lemma OclIsTypeOf\<^sub>P\<^sub>e\<^sub>r\<^sub>s\<^sub>o\<^sub>n_Galaxy_defined : 
 assumes isdef: "\<tau> \<Turnstile> (\<upsilon> (X))"
 shows "\<tau> \<Turnstile> (\<delta> ((X::Galaxy) .oclIsTypeOf(Person)))"
   apply(insert isdef[simplified foundation18'], simp only: OclValid_def, subst cp_defined)
-by(auto simp: cp_defined[symmetric ] bot_option_def OclIsTypeOf\<^sub>P\<^sub>e\<^sub>r\<^sub>s\<^sub>o\<^sub>n_Galaxy split: option.split type\<^sub>G\<^sub>a\<^sub>l\<^sub>a\<^sub>x\<^sub>y.split typeoid\<^sub>G\<^sub>a\<^sub>l\<^sub>a\<^sub>x\<^sub>y.split) 
+by(auto simp: cp_defined[symmetric ] bot_option_def OclIsTypeOf\<^sub>P\<^sub>e\<^sub>r\<^sub>s\<^sub>o\<^sub>n_Galaxy split: option.split ty\<E>\<X>\<T>\<^sub>G\<^sub>a\<^sub>l\<^sub>a\<^sub>x\<^sub>y.split ty\<^sub>G\<^sub>a\<^sub>l\<^sub>a\<^sub>x\<^sub>y.split) 
 lemma OclIsTypeOf\<^sub>P\<^sub>e\<^sub>r\<^sub>s\<^sub>o\<^sub>n_OclAny_defined : 
 assumes isdef: "\<tau> \<Turnstile> (\<upsilon> (X))"
 shows "\<tau> \<Turnstile> (\<delta> ((X::OclAny) .oclIsTypeOf(Person)))"
   apply(insert isdef[simplified foundation18'], simp only: OclValid_def, subst cp_defined)
-by(auto simp: cp_defined[symmetric ] bot_option_def OclIsTypeOf\<^sub>P\<^sub>e\<^sub>r\<^sub>s\<^sub>o\<^sub>n_OclAny split: option.split type\<^sub>O\<^sub>c\<^sub>l\<^sub>A\<^sub>n\<^sub>y.split typeoid\<^sub>O\<^sub>c\<^sub>l\<^sub>A\<^sub>n\<^sub>y.split) 
+by(auto simp: cp_defined[symmetric ] bot_option_def OclIsTypeOf\<^sub>P\<^sub>e\<^sub>r\<^sub>s\<^sub>o\<^sub>n_OclAny split: option.split ty\<E>\<X>\<T>\<^sub>O\<^sub>c\<^sub>l\<^sub>A\<^sub>n\<^sub>y.split ty\<^sub>O\<^sub>c\<^sub>l\<^sub>A\<^sub>n\<^sub>y.split) 
 lemma OclIsTypeOf\<^sub>P\<^sub>l\<^sub>a\<^sub>n\<^sub>e\<^sub>t_Planet_defined : 
 assumes isdef: "\<tau> \<Turnstile> (\<upsilon> (X))"
 shows "\<tau> \<Turnstile> (\<delta> ((X::Planet) .oclIsTypeOf(Planet)))"
   apply(insert isdef[simplified foundation18'], simp only: OclValid_def, subst cp_defined)
-by(auto simp: cp_defined[symmetric ] bot_option_def OclIsTypeOf\<^sub>P\<^sub>l\<^sub>a\<^sub>n\<^sub>e\<^sub>t_Planet split: option.split type\<^sub>P\<^sub>l\<^sub>a\<^sub>n\<^sub>e\<^sub>t.split typeoid\<^sub>P\<^sub>l\<^sub>a\<^sub>n\<^sub>e\<^sub>t.split) 
+by(auto simp: cp_defined[symmetric ] bot_option_def OclIsTypeOf\<^sub>P\<^sub>l\<^sub>a\<^sub>n\<^sub>e\<^sub>t_Planet split: option.split ty\<E>\<X>\<T>\<^sub>P\<^sub>l\<^sub>a\<^sub>n\<^sub>e\<^sub>t.split ty\<^sub>P\<^sub>l\<^sub>a\<^sub>n\<^sub>e\<^sub>t.split) 
 lemma OclIsTypeOf\<^sub>P\<^sub>l\<^sub>a\<^sub>n\<^sub>e\<^sub>t_Galaxy_defined : 
 assumes isdef: "\<tau> \<Turnstile> (\<upsilon> (X))"
 shows "\<tau> \<Turnstile> (\<delta> ((X::Galaxy) .oclIsTypeOf(Planet)))"
   apply(insert isdef[simplified foundation18'], simp only: OclValid_def, subst cp_defined)
-by(auto simp: cp_defined[symmetric ] bot_option_def OclIsTypeOf\<^sub>P\<^sub>l\<^sub>a\<^sub>n\<^sub>e\<^sub>t_Galaxy split: option.split type\<^sub>G\<^sub>a\<^sub>l\<^sub>a\<^sub>x\<^sub>y.split typeoid\<^sub>G\<^sub>a\<^sub>l\<^sub>a\<^sub>x\<^sub>y.split) 
+by(auto simp: cp_defined[symmetric ] bot_option_def OclIsTypeOf\<^sub>P\<^sub>l\<^sub>a\<^sub>n\<^sub>e\<^sub>t_Galaxy split: option.split ty\<E>\<X>\<T>\<^sub>G\<^sub>a\<^sub>l\<^sub>a\<^sub>x\<^sub>y.split ty\<^sub>G\<^sub>a\<^sub>l\<^sub>a\<^sub>x\<^sub>y.split) 
 lemma OclIsTypeOf\<^sub>P\<^sub>l\<^sub>a\<^sub>n\<^sub>e\<^sub>t_OclAny_defined : 
 assumes isdef: "\<tau> \<Turnstile> (\<upsilon> (X))"
 shows "\<tau> \<Turnstile> (\<delta> ((X::OclAny) .oclIsTypeOf(Planet)))"
   apply(insert isdef[simplified foundation18'], simp only: OclValid_def, subst cp_defined)
-by(auto simp: cp_defined[symmetric ] bot_option_def OclIsTypeOf\<^sub>P\<^sub>l\<^sub>a\<^sub>n\<^sub>e\<^sub>t_OclAny split: option.split type\<^sub>O\<^sub>c\<^sub>l\<^sub>A\<^sub>n\<^sub>y.split typeoid\<^sub>O\<^sub>c\<^sub>l\<^sub>A\<^sub>n\<^sub>y.split) 
+by(auto simp: cp_defined[symmetric ] bot_option_def OclIsTypeOf\<^sub>P\<^sub>l\<^sub>a\<^sub>n\<^sub>e\<^sub>t_OclAny split: option.split ty\<E>\<X>\<T>\<^sub>O\<^sub>c\<^sub>l\<^sub>A\<^sub>n\<^sub>y.split ty\<^sub>O\<^sub>c\<^sub>l\<^sub>A\<^sub>n\<^sub>y.split) 
 lemma OclIsTypeOf\<^sub>P\<^sub>l\<^sub>a\<^sub>n\<^sub>e\<^sub>t_Person_defined : 
 assumes isdef: "\<tau> \<Turnstile> (\<upsilon> (X))"
 shows "\<tau> \<Turnstile> (\<delta> ((X::Person) .oclIsTypeOf(Planet)))"
   apply(insert isdef[simplified foundation18'], simp only: OclValid_def, subst cp_defined)
-by(auto simp: cp_defined[symmetric ] bot_option_def OclIsTypeOf\<^sub>P\<^sub>l\<^sub>a\<^sub>n\<^sub>e\<^sub>t_Person split: option.split type\<^sub>P\<^sub>e\<^sub>r\<^sub>s\<^sub>o\<^sub>n.split typeoid\<^sub>P\<^sub>e\<^sub>r\<^sub>s\<^sub>o\<^sub>n.split) 
+by(auto simp: cp_defined[symmetric ] bot_option_def OclIsTypeOf\<^sub>P\<^sub>l\<^sub>a\<^sub>n\<^sub>e\<^sub>t_Person split: option.split ty\<E>\<X>\<T>\<^sub>P\<^sub>e\<^sub>r\<^sub>s\<^sub>o\<^sub>n.split ty\<^sub>P\<^sub>e\<^sub>r\<^sub>s\<^sub>o\<^sub>n.split) 
 lemma OclIsTypeOf\<^sub>G\<^sub>a\<^sub>l\<^sub>a\<^sub>x\<^sub>y_Galaxy_defined : 
 assumes isdef: "\<tau> \<Turnstile> (\<upsilon> (X))"
 shows "\<tau> \<Turnstile> (\<delta> ((X::Galaxy) .oclIsTypeOf(Galaxy)))"
   apply(insert isdef[simplified foundation18'], simp only: OclValid_def, subst cp_defined)
-by(auto simp: cp_defined[symmetric ] bot_option_def OclIsTypeOf\<^sub>G\<^sub>a\<^sub>l\<^sub>a\<^sub>x\<^sub>y_Galaxy split: option.split type\<^sub>G\<^sub>a\<^sub>l\<^sub>a\<^sub>x\<^sub>y.split typeoid\<^sub>G\<^sub>a\<^sub>l\<^sub>a\<^sub>x\<^sub>y.split) 
+by(auto simp: cp_defined[symmetric ] bot_option_def OclIsTypeOf\<^sub>G\<^sub>a\<^sub>l\<^sub>a\<^sub>x\<^sub>y_Galaxy split: option.split ty\<E>\<X>\<T>\<^sub>G\<^sub>a\<^sub>l\<^sub>a\<^sub>x\<^sub>y.split ty\<^sub>G\<^sub>a\<^sub>l\<^sub>a\<^sub>x\<^sub>y.split) 
 lemma OclIsTypeOf\<^sub>G\<^sub>a\<^sub>l\<^sub>a\<^sub>x\<^sub>y_OclAny_defined : 
 assumes isdef: "\<tau> \<Turnstile> (\<upsilon> (X))"
 shows "\<tau> \<Turnstile> (\<delta> ((X::OclAny) .oclIsTypeOf(Galaxy)))"
   apply(insert isdef[simplified foundation18'], simp only: OclValid_def, subst cp_defined)
-by(auto simp: cp_defined[symmetric ] bot_option_def OclIsTypeOf\<^sub>G\<^sub>a\<^sub>l\<^sub>a\<^sub>x\<^sub>y_OclAny split: option.split type\<^sub>O\<^sub>c\<^sub>l\<^sub>A\<^sub>n\<^sub>y.split typeoid\<^sub>O\<^sub>c\<^sub>l\<^sub>A\<^sub>n\<^sub>y.split) 
+by(auto simp: cp_defined[symmetric ] bot_option_def OclIsTypeOf\<^sub>G\<^sub>a\<^sub>l\<^sub>a\<^sub>x\<^sub>y_OclAny split: option.split ty\<E>\<X>\<T>\<^sub>O\<^sub>c\<^sub>l\<^sub>A\<^sub>n\<^sub>y.split ty\<^sub>O\<^sub>c\<^sub>l\<^sub>A\<^sub>n\<^sub>y.split) 
 lemma OclIsTypeOf\<^sub>G\<^sub>a\<^sub>l\<^sub>a\<^sub>x\<^sub>y_Person_defined : 
 assumes isdef: "\<tau> \<Turnstile> (\<upsilon> (X))"
 shows "\<tau> \<Turnstile> (\<delta> ((X::Person) .oclIsTypeOf(Galaxy)))"
   apply(insert isdef[simplified foundation18'], simp only: OclValid_def, subst cp_defined)
-by(auto simp: cp_defined[symmetric ] bot_option_def OclIsTypeOf\<^sub>G\<^sub>a\<^sub>l\<^sub>a\<^sub>x\<^sub>y_Person split: option.split type\<^sub>P\<^sub>e\<^sub>r\<^sub>s\<^sub>o\<^sub>n.split typeoid\<^sub>P\<^sub>e\<^sub>r\<^sub>s\<^sub>o\<^sub>n.split) 
+by(auto simp: cp_defined[symmetric ] bot_option_def OclIsTypeOf\<^sub>G\<^sub>a\<^sub>l\<^sub>a\<^sub>x\<^sub>y_Person split: option.split ty\<E>\<X>\<T>\<^sub>P\<^sub>e\<^sub>r\<^sub>s\<^sub>o\<^sub>n.split ty\<^sub>P\<^sub>e\<^sub>r\<^sub>s\<^sub>o\<^sub>n.split) 
 lemma OclIsTypeOf\<^sub>G\<^sub>a\<^sub>l\<^sub>a\<^sub>x\<^sub>y_Planet_defined : 
 assumes isdef: "\<tau> \<Turnstile> (\<upsilon> (X))"
 shows "\<tau> \<Turnstile> (\<delta> ((X::Planet) .oclIsTypeOf(Galaxy)))"
   apply(insert isdef[simplified foundation18'], simp only: OclValid_def, subst cp_defined)
-by(auto simp: cp_defined[symmetric ] bot_option_def OclIsTypeOf\<^sub>G\<^sub>a\<^sub>l\<^sub>a\<^sub>x\<^sub>y_Planet split: option.split type\<^sub>P\<^sub>l\<^sub>a\<^sub>n\<^sub>e\<^sub>t.split typeoid\<^sub>P\<^sub>l\<^sub>a\<^sub>n\<^sub>e\<^sub>t.split) 
+by(auto simp: cp_defined[symmetric ] bot_option_def OclIsTypeOf\<^sub>G\<^sub>a\<^sub>l\<^sub>a\<^sub>x\<^sub>y_Planet split: option.split ty\<E>\<X>\<T>\<^sub>P\<^sub>l\<^sub>a\<^sub>n\<^sub>e\<^sub>t.split ty\<^sub>P\<^sub>l\<^sub>a\<^sub>n\<^sub>e\<^sub>t.split) 
 lemma OclIsTypeOf\<^sub>O\<^sub>c\<^sub>l\<^sub>A\<^sub>n\<^sub>y_OclAny_defined : 
 assumes isdef: "\<tau> \<Turnstile> (\<upsilon> (X))"
 shows "\<tau> \<Turnstile> (\<delta> ((X::OclAny) .oclIsTypeOf(OclAny)))"
   apply(insert isdef[simplified foundation18'], simp only: OclValid_def, subst cp_defined)
-by(auto simp: cp_defined[symmetric ] bot_option_def OclIsTypeOf\<^sub>O\<^sub>c\<^sub>l\<^sub>A\<^sub>n\<^sub>y_OclAny split: option.split type\<^sub>O\<^sub>c\<^sub>l\<^sub>A\<^sub>n\<^sub>y.split typeoid\<^sub>O\<^sub>c\<^sub>l\<^sub>A\<^sub>n\<^sub>y.split) 
+by(auto simp: cp_defined[symmetric ] bot_option_def OclIsTypeOf\<^sub>O\<^sub>c\<^sub>l\<^sub>A\<^sub>n\<^sub>y_OclAny split: option.split ty\<E>\<X>\<T>\<^sub>O\<^sub>c\<^sub>l\<^sub>A\<^sub>n\<^sub>y.split ty\<^sub>O\<^sub>c\<^sub>l\<^sub>A\<^sub>n\<^sub>y.split) 
 lemma OclIsTypeOf\<^sub>O\<^sub>c\<^sub>l\<^sub>A\<^sub>n\<^sub>y_Person_defined : 
 assumes isdef: "\<tau> \<Turnstile> (\<upsilon> (X))"
 shows "\<tau> \<Turnstile> (\<delta> ((X::Person) .oclIsTypeOf(OclAny)))"
   apply(insert isdef[simplified foundation18'], simp only: OclValid_def, subst cp_defined)
-by(auto simp: cp_defined[symmetric ] bot_option_def OclIsTypeOf\<^sub>O\<^sub>c\<^sub>l\<^sub>A\<^sub>n\<^sub>y_Person split: option.split type\<^sub>P\<^sub>e\<^sub>r\<^sub>s\<^sub>o\<^sub>n.split typeoid\<^sub>P\<^sub>e\<^sub>r\<^sub>s\<^sub>o\<^sub>n.split) 
+by(auto simp: cp_defined[symmetric ] bot_option_def OclIsTypeOf\<^sub>O\<^sub>c\<^sub>l\<^sub>A\<^sub>n\<^sub>y_Person split: option.split ty\<E>\<X>\<T>\<^sub>P\<^sub>e\<^sub>r\<^sub>s\<^sub>o\<^sub>n.split ty\<^sub>P\<^sub>e\<^sub>r\<^sub>s\<^sub>o\<^sub>n.split) 
 lemma OclIsTypeOf\<^sub>O\<^sub>c\<^sub>l\<^sub>A\<^sub>n\<^sub>y_Planet_defined : 
 assumes isdef: "\<tau> \<Turnstile> (\<upsilon> (X))"
 shows "\<tau> \<Turnstile> (\<delta> ((X::Planet) .oclIsTypeOf(OclAny)))"
   apply(insert isdef[simplified foundation18'], simp only: OclValid_def, subst cp_defined)
-by(auto simp: cp_defined[symmetric ] bot_option_def OclIsTypeOf\<^sub>O\<^sub>c\<^sub>l\<^sub>A\<^sub>n\<^sub>y_Planet split: option.split type\<^sub>P\<^sub>l\<^sub>a\<^sub>n\<^sub>e\<^sub>t.split typeoid\<^sub>P\<^sub>l\<^sub>a\<^sub>n\<^sub>e\<^sub>t.split) 
+by(auto simp: cp_defined[symmetric ] bot_option_def OclIsTypeOf\<^sub>O\<^sub>c\<^sub>l\<^sub>A\<^sub>n\<^sub>y_Planet split: option.split ty\<E>\<X>\<T>\<^sub>P\<^sub>l\<^sub>a\<^sub>n\<^sub>e\<^sub>t.split ty\<^sub>P\<^sub>l\<^sub>a\<^sub>n\<^sub>e\<^sub>t.split) 
 lemma OclIsTypeOf\<^sub>O\<^sub>c\<^sub>l\<^sub>A\<^sub>n\<^sub>y_Galaxy_defined : 
 assumes isdef: "\<tau> \<Turnstile> (\<upsilon> (X))"
 shows "\<tau> \<Turnstile> (\<delta> ((X::Galaxy) .oclIsTypeOf(OclAny)))"
   apply(insert isdef[simplified foundation18'], simp only: OclValid_def, subst cp_defined)
-by(auto simp: cp_defined[symmetric ] bot_option_def OclIsTypeOf\<^sub>O\<^sub>c\<^sub>l\<^sub>A\<^sub>n\<^sub>y_Galaxy split: option.split type\<^sub>G\<^sub>a\<^sub>l\<^sub>a\<^sub>x\<^sub>y.split typeoid\<^sub>G\<^sub>a\<^sub>l\<^sub>a\<^sub>x\<^sub>y.split) 
+by(auto simp: cp_defined[symmetric ] bot_option_def OclIsTypeOf\<^sub>O\<^sub>c\<^sub>l\<^sub>A\<^sub>n\<^sub>y_Galaxy split: option.split ty\<E>\<X>\<T>\<^sub>G\<^sub>a\<^sub>l\<^sub>a\<^sub>x\<^sub>y.split ty\<^sub>G\<^sub>a\<^sub>l\<^sub>a\<^sub>x\<^sub>y.split) 
 
 (* 61 ************************************ 348 + 16 *)
 lemma OclIsTypeOf\<^sub>P\<^sub>e\<^sub>r\<^sub>s\<^sub>o\<^sub>n_Person_defined' : 
@@ -1332,70 +1332,70 @@ assumes istyp: "\<tau> \<Turnstile> ((X::Planet) .oclIsTypeOf(Planet))"
 assumes isdef: "\<tau> \<Turnstile> (\<delta> (X))"
 shows "\<tau> \<Turnstile> (X .oclAsType(Person)) \<triangleq> invalid"
   using istyp isdef
-  apply(auto simp: OclAsType\<^sub>P\<^sub>e\<^sub>r\<^sub>s\<^sub>o\<^sub>n_Planet foundation22 foundation16 null_option_def bot_option_def split: type\<^sub>P\<^sub>l\<^sub>a\<^sub>n\<^sub>e\<^sub>t.split typeoid\<^sub>P\<^sub>l\<^sub>a\<^sub>n\<^sub>e\<^sub>t.split)
+  apply(auto simp: OclAsType\<^sub>P\<^sub>e\<^sub>r\<^sub>s\<^sub>o\<^sub>n_Planet foundation22 foundation16 null_option_def bot_option_def split: ty\<E>\<X>\<T>\<^sub>P\<^sub>l\<^sub>a\<^sub>n\<^sub>e\<^sub>t.split ty\<^sub>P\<^sub>l\<^sub>a\<^sub>n\<^sub>e\<^sub>t.split)
 by(simp add: OclValid_def false_def true_def) 
 lemma down_cast_type\<^sub>G\<^sub>a\<^sub>l\<^sub>a\<^sub>x\<^sub>y_from_Galaxy_to_Person : 
 assumes istyp: "\<tau> \<Turnstile> ((X::Galaxy) .oclIsTypeOf(Galaxy))"
 assumes isdef: "\<tau> \<Turnstile> (\<delta> (X))"
 shows "\<tau> \<Turnstile> (X .oclAsType(Person)) \<triangleq> invalid"
   using istyp isdef
-  apply(auto simp: OclAsType\<^sub>P\<^sub>e\<^sub>r\<^sub>s\<^sub>o\<^sub>n_Galaxy foundation22 foundation16 null_option_def bot_option_def split: type\<^sub>G\<^sub>a\<^sub>l\<^sub>a\<^sub>x\<^sub>y.split typeoid\<^sub>G\<^sub>a\<^sub>l\<^sub>a\<^sub>x\<^sub>y.split)
+  apply(auto simp: OclAsType\<^sub>P\<^sub>e\<^sub>r\<^sub>s\<^sub>o\<^sub>n_Galaxy foundation22 foundation16 null_option_def bot_option_def split: ty\<E>\<X>\<T>\<^sub>G\<^sub>a\<^sub>l\<^sub>a\<^sub>x\<^sub>y.split ty\<^sub>G\<^sub>a\<^sub>l\<^sub>a\<^sub>x\<^sub>y.split)
 by(simp add: OclValid_def false_def true_def) 
 lemma down_cast_type\<^sub>O\<^sub>c\<^sub>l\<^sub>A\<^sub>n\<^sub>y_from_OclAny_to_Person : 
 assumes istyp: "\<tau> \<Turnstile> ((X::OclAny) .oclIsTypeOf(OclAny))"
 assumes isdef: "\<tau> \<Turnstile> (\<delta> (X))"
 shows "\<tau> \<Turnstile> (X .oclAsType(Person)) \<triangleq> invalid"
   using istyp isdef
-  apply(auto simp: OclAsType\<^sub>P\<^sub>e\<^sub>r\<^sub>s\<^sub>o\<^sub>n_OclAny foundation22 foundation16 null_option_def bot_option_def split: type\<^sub>O\<^sub>c\<^sub>l\<^sub>A\<^sub>n\<^sub>y.split typeoid\<^sub>O\<^sub>c\<^sub>l\<^sub>A\<^sub>n\<^sub>y.split)
+  apply(auto simp: OclAsType\<^sub>P\<^sub>e\<^sub>r\<^sub>s\<^sub>o\<^sub>n_OclAny foundation22 foundation16 null_option_def bot_option_def split: ty\<E>\<X>\<T>\<^sub>O\<^sub>c\<^sub>l\<^sub>A\<^sub>n\<^sub>y.split ty\<^sub>O\<^sub>c\<^sub>l\<^sub>A\<^sub>n\<^sub>y.split)
 by(simp add: OclValid_def false_def true_def) 
 lemma down_cast_type\<^sub>P\<^sub>l\<^sub>a\<^sub>n\<^sub>e\<^sub>t_from_Galaxy_to_Person : 
 assumes istyp: "\<tau> \<Turnstile> ((X::Galaxy) .oclIsTypeOf(Planet))"
 assumes isdef: "\<tau> \<Turnstile> (\<delta> (X))"
 shows "\<tau> \<Turnstile> (X .oclAsType(Person)) \<triangleq> invalid"
   using istyp isdef
-  apply(auto simp: OclAsType\<^sub>P\<^sub>e\<^sub>r\<^sub>s\<^sub>o\<^sub>n_Galaxy foundation22 foundation16 null_option_def bot_option_def split: type\<^sub>G\<^sub>a\<^sub>l\<^sub>a\<^sub>x\<^sub>y.split typeoid\<^sub>G\<^sub>a\<^sub>l\<^sub>a\<^sub>x\<^sub>y.split)
+  apply(auto simp: OclAsType\<^sub>P\<^sub>e\<^sub>r\<^sub>s\<^sub>o\<^sub>n_Galaxy foundation22 foundation16 null_option_def bot_option_def split: ty\<E>\<X>\<T>\<^sub>G\<^sub>a\<^sub>l\<^sub>a\<^sub>x\<^sub>y.split ty\<^sub>G\<^sub>a\<^sub>l\<^sub>a\<^sub>x\<^sub>y.split)
 by(simp add: OclIsTypeOf\<^sub>P\<^sub>l\<^sub>a\<^sub>n\<^sub>e\<^sub>t_Galaxy OclValid_def false_def true_def) 
 lemma down_cast_type\<^sub>P\<^sub>l\<^sub>a\<^sub>n\<^sub>e\<^sub>t_from_OclAny_to_Person : 
 assumes istyp: "\<tau> \<Turnstile> ((X::OclAny) .oclIsTypeOf(Planet))"
 assumes isdef: "\<tau> \<Turnstile> (\<delta> (X))"
 shows "\<tau> \<Turnstile> (X .oclAsType(Person)) \<triangleq> invalid"
   using istyp isdef
-  apply(auto simp: OclAsType\<^sub>P\<^sub>e\<^sub>r\<^sub>s\<^sub>o\<^sub>n_OclAny foundation22 foundation16 null_option_def bot_option_def split: type\<^sub>O\<^sub>c\<^sub>l\<^sub>A\<^sub>n\<^sub>y.split typeoid\<^sub>O\<^sub>c\<^sub>l\<^sub>A\<^sub>n\<^sub>y.split)
+  apply(auto simp: OclAsType\<^sub>P\<^sub>e\<^sub>r\<^sub>s\<^sub>o\<^sub>n_OclAny foundation22 foundation16 null_option_def bot_option_def split: ty\<E>\<X>\<T>\<^sub>O\<^sub>c\<^sub>l\<^sub>A\<^sub>n\<^sub>y.split ty\<^sub>O\<^sub>c\<^sub>l\<^sub>A\<^sub>n\<^sub>y.split)
 by(simp add: OclIsTypeOf\<^sub>P\<^sub>l\<^sub>a\<^sub>n\<^sub>e\<^sub>t_OclAny OclValid_def false_def true_def) 
 lemma down_cast_type\<^sub>G\<^sub>a\<^sub>l\<^sub>a\<^sub>x\<^sub>y_from_OclAny_to_Person : 
 assumes istyp: "\<tau> \<Turnstile> ((X::OclAny) .oclIsTypeOf(Galaxy))"
 assumes isdef: "\<tau> \<Turnstile> (\<delta> (X))"
 shows "\<tau> \<Turnstile> (X .oclAsType(Person)) \<triangleq> invalid"
   using istyp isdef
-  apply(auto simp: OclAsType\<^sub>P\<^sub>e\<^sub>r\<^sub>s\<^sub>o\<^sub>n_OclAny foundation22 foundation16 null_option_def bot_option_def split: type\<^sub>O\<^sub>c\<^sub>l\<^sub>A\<^sub>n\<^sub>y.split typeoid\<^sub>O\<^sub>c\<^sub>l\<^sub>A\<^sub>n\<^sub>y.split)
+  apply(auto simp: OclAsType\<^sub>P\<^sub>e\<^sub>r\<^sub>s\<^sub>o\<^sub>n_OclAny foundation22 foundation16 null_option_def bot_option_def split: ty\<E>\<X>\<T>\<^sub>O\<^sub>c\<^sub>l\<^sub>A\<^sub>n\<^sub>y.split ty\<^sub>O\<^sub>c\<^sub>l\<^sub>A\<^sub>n\<^sub>y.split)
 by(simp add: OclIsTypeOf\<^sub>G\<^sub>a\<^sub>l\<^sub>a\<^sub>x\<^sub>y_OclAny OclValid_def false_def true_def) 
 lemma down_cast_type\<^sub>G\<^sub>a\<^sub>l\<^sub>a\<^sub>x\<^sub>y_from_Galaxy_to_Planet : 
 assumes istyp: "\<tau> \<Turnstile> ((X::Galaxy) .oclIsTypeOf(Galaxy))"
 assumes isdef: "\<tau> \<Turnstile> (\<delta> (X))"
 shows "\<tau> \<Turnstile> (X .oclAsType(Planet)) \<triangleq> invalid"
   using istyp isdef
-  apply(auto simp: OclAsType\<^sub>P\<^sub>l\<^sub>a\<^sub>n\<^sub>e\<^sub>t_Galaxy foundation22 foundation16 null_option_def bot_option_def split: type\<^sub>G\<^sub>a\<^sub>l\<^sub>a\<^sub>x\<^sub>y.split typeoid\<^sub>G\<^sub>a\<^sub>l\<^sub>a\<^sub>x\<^sub>y.split)
+  apply(auto simp: OclAsType\<^sub>P\<^sub>l\<^sub>a\<^sub>n\<^sub>e\<^sub>t_Galaxy foundation22 foundation16 null_option_def bot_option_def split: ty\<E>\<X>\<T>\<^sub>G\<^sub>a\<^sub>l\<^sub>a\<^sub>x\<^sub>y.split ty\<^sub>G\<^sub>a\<^sub>l\<^sub>a\<^sub>x\<^sub>y.split)
 by(simp add: OclValid_def false_def true_def) 
 lemma down_cast_type\<^sub>O\<^sub>c\<^sub>l\<^sub>A\<^sub>n\<^sub>y_from_OclAny_to_Planet : 
 assumes istyp: "\<tau> \<Turnstile> ((X::OclAny) .oclIsTypeOf(OclAny))"
 assumes isdef: "\<tau> \<Turnstile> (\<delta> (X))"
 shows "\<tau> \<Turnstile> (X .oclAsType(Planet)) \<triangleq> invalid"
   using istyp isdef
-  apply(auto simp: OclAsType\<^sub>P\<^sub>l\<^sub>a\<^sub>n\<^sub>e\<^sub>t_OclAny foundation22 foundation16 null_option_def bot_option_def split: type\<^sub>O\<^sub>c\<^sub>l\<^sub>A\<^sub>n\<^sub>y.split typeoid\<^sub>O\<^sub>c\<^sub>l\<^sub>A\<^sub>n\<^sub>y.split)
+  apply(auto simp: OclAsType\<^sub>P\<^sub>l\<^sub>a\<^sub>n\<^sub>e\<^sub>t_OclAny foundation22 foundation16 null_option_def bot_option_def split: ty\<E>\<X>\<T>\<^sub>O\<^sub>c\<^sub>l\<^sub>A\<^sub>n\<^sub>y.split ty\<^sub>O\<^sub>c\<^sub>l\<^sub>A\<^sub>n\<^sub>y.split)
 by(simp add: OclValid_def false_def true_def) 
 lemma down_cast_type\<^sub>G\<^sub>a\<^sub>l\<^sub>a\<^sub>x\<^sub>y_from_OclAny_to_Planet : 
 assumes istyp: "\<tau> \<Turnstile> ((X::OclAny) .oclIsTypeOf(Galaxy))"
 assumes isdef: "\<tau> \<Turnstile> (\<delta> (X))"
 shows "\<tau> \<Turnstile> (X .oclAsType(Planet)) \<triangleq> invalid"
   using istyp isdef
-  apply(auto simp: OclAsType\<^sub>P\<^sub>l\<^sub>a\<^sub>n\<^sub>e\<^sub>t_OclAny foundation22 foundation16 null_option_def bot_option_def split: type\<^sub>O\<^sub>c\<^sub>l\<^sub>A\<^sub>n\<^sub>y.split typeoid\<^sub>O\<^sub>c\<^sub>l\<^sub>A\<^sub>n\<^sub>y.split)
+  apply(auto simp: OclAsType\<^sub>P\<^sub>l\<^sub>a\<^sub>n\<^sub>e\<^sub>t_OclAny foundation22 foundation16 null_option_def bot_option_def split: ty\<E>\<X>\<T>\<^sub>O\<^sub>c\<^sub>l\<^sub>A\<^sub>n\<^sub>y.split ty\<^sub>O\<^sub>c\<^sub>l\<^sub>A\<^sub>n\<^sub>y.split)
 by(simp add: OclIsTypeOf\<^sub>G\<^sub>a\<^sub>l\<^sub>a\<^sub>x\<^sub>y_OclAny OclValid_def false_def true_def) 
 lemma down_cast_type\<^sub>O\<^sub>c\<^sub>l\<^sub>A\<^sub>n\<^sub>y_from_OclAny_to_Galaxy : 
 assumes istyp: "\<tau> \<Turnstile> ((X::OclAny) .oclIsTypeOf(OclAny))"
 assumes isdef: "\<tau> \<Turnstile> (\<delta> (X))"
 shows "\<tau> \<Turnstile> (X .oclAsType(Galaxy)) \<triangleq> invalid"
   using istyp isdef
-  apply(auto simp: OclAsType\<^sub>G\<^sub>a\<^sub>l\<^sub>a\<^sub>x\<^sub>y_OclAny foundation22 foundation16 null_option_def bot_option_def split: type\<^sub>O\<^sub>c\<^sub>l\<^sub>A\<^sub>n\<^sub>y.split typeoid\<^sub>O\<^sub>c\<^sub>l\<^sub>A\<^sub>n\<^sub>y.split)
+  apply(auto simp: OclAsType\<^sub>G\<^sub>a\<^sub>l\<^sub>a\<^sub>x\<^sub>y_OclAny foundation22 foundation16 null_option_def bot_option_def split: ty\<E>\<X>\<T>\<^sub>O\<^sub>c\<^sub>l\<^sub>A\<^sub>n\<^sub>y.split ty\<^sub>O\<^sub>c\<^sub>l\<^sub>A\<^sub>n\<^sub>y.split)
 by(simp add: OclValid_def false_def true_def) 
 
 (* 65 ************************************ 381 + 1 *)
@@ -2042,28 +2042,28 @@ assumes isdef: "\<tau> \<Turnstile> (\<delta> (X))"
 shows "\<tau> \<Turnstile> ((X::Person) .oclIsKindOf(Person))"
   apply(simp only: OclValid_def, insert isdef)
   apply(simp only: OclIsKindOf\<^sub>P\<^sub>e\<^sub>r\<^sub>s\<^sub>o\<^sub>n_Person)
-  apply(auto simp: foundation16 bot_option_def split: option.split type\<^sub>P\<^sub>e\<^sub>r\<^sub>s\<^sub>o\<^sub>n.split typeoid\<^sub>P\<^sub>e\<^sub>r\<^sub>s\<^sub>o\<^sub>n.split)
+  apply(auto simp: foundation16 bot_option_def split: option.split ty\<E>\<X>\<T>\<^sub>P\<^sub>e\<^sub>r\<^sub>s\<^sub>o\<^sub>n.split ty\<^sub>P\<^sub>e\<^sub>r\<^sub>s\<^sub>o\<^sub>n.split)
 by((simp_all add: false_def true_def OclOr_def OclAnd_def OclNot_def)?) 
 lemma actual_eq_static\<^sub>P\<^sub>l\<^sub>a\<^sub>n\<^sub>e\<^sub>t : 
 assumes isdef: "\<tau> \<Turnstile> (\<delta> (X))"
 shows "\<tau> \<Turnstile> ((X::Planet) .oclIsKindOf(Planet))"
   apply(simp only: OclValid_def, insert isdef)
   apply(simp only: OclIsKindOf\<^sub>P\<^sub>l\<^sub>a\<^sub>n\<^sub>e\<^sub>t_Planet, subst (1) cp_OclOr, simp only: OclIsKindOf\<^sub>P\<^sub>e\<^sub>r\<^sub>s\<^sub>o\<^sub>n_Planet)
-  apply(auto simp: cp_OclOr[symmetric ] foundation16 bot_option_def OclIsTypeOf\<^sub>P\<^sub>e\<^sub>r\<^sub>s\<^sub>o\<^sub>n_Planet split: option.split type\<^sub>P\<^sub>l\<^sub>a\<^sub>n\<^sub>e\<^sub>t.split typeoid\<^sub>P\<^sub>l\<^sub>a\<^sub>n\<^sub>e\<^sub>t.split type\<^sub>P\<^sub>e\<^sub>r\<^sub>s\<^sub>o\<^sub>n.split typeoid\<^sub>P\<^sub>e\<^sub>r\<^sub>s\<^sub>o\<^sub>n.split)
+  apply(auto simp: cp_OclOr[symmetric ] foundation16 bot_option_def OclIsTypeOf\<^sub>P\<^sub>e\<^sub>r\<^sub>s\<^sub>o\<^sub>n_Planet split: option.split ty\<E>\<X>\<T>\<^sub>P\<^sub>l\<^sub>a\<^sub>n\<^sub>e\<^sub>t.split ty\<^sub>P\<^sub>l\<^sub>a\<^sub>n\<^sub>e\<^sub>t.split ty\<E>\<X>\<T>\<^sub>P\<^sub>e\<^sub>r\<^sub>s\<^sub>o\<^sub>n.split ty\<^sub>P\<^sub>e\<^sub>r\<^sub>s\<^sub>o\<^sub>n.split)
 by((simp_all add: false_def true_def OclOr_def OclAnd_def OclNot_def)?) 
 lemma actual_eq_static\<^sub>G\<^sub>a\<^sub>l\<^sub>a\<^sub>x\<^sub>y : 
 assumes isdef: "\<tau> \<Turnstile> (\<delta> (X))"
 shows "\<tau> \<Turnstile> ((X::Galaxy) .oclIsKindOf(Galaxy))"
   apply(simp only: OclValid_def, insert isdef)
   apply(simp only: OclIsKindOf\<^sub>G\<^sub>a\<^sub>l\<^sub>a\<^sub>x\<^sub>y_Galaxy, subst (1) cp_OclOr, simp only: OclIsKindOf\<^sub>P\<^sub>l\<^sub>a\<^sub>n\<^sub>e\<^sub>t_Galaxy, subst (2 1) cp_OclOr, simp only: OclIsKindOf\<^sub>P\<^sub>e\<^sub>r\<^sub>s\<^sub>o\<^sub>n_Galaxy)
-  apply(auto simp: cp_OclOr[symmetric ] foundation16 bot_option_def OclIsTypeOf\<^sub>P\<^sub>e\<^sub>r\<^sub>s\<^sub>o\<^sub>n_Galaxy OclIsTypeOf\<^sub>P\<^sub>l\<^sub>a\<^sub>n\<^sub>e\<^sub>t_Galaxy split: option.split type\<^sub>G\<^sub>a\<^sub>l\<^sub>a\<^sub>x\<^sub>y.split typeoid\<^sub>G\<^sub>a\<^sub>l\<^sub>a\<^sub>x\<^sub>y.split type\<^sub>P\<^sub>e\<^sub>r\<^sub>s\<^sub>o\<^sub>n.split typeoid\<^sub>P\<^sub>e\<^sub>r\<^sub>s\<^sub>o\<^sub>n.split type\<^sub>P\<^sub>l\<^sub>a\<^sub>n\<^sub>e\<^sub>t.split typeoid\<^sub>P\<^sub>l\<^sub>a\<^sub>n\<^sub>e\<^sub>t.split)
+  apply(auto simp: cp_OclOr[symmetric ] foundation16 bot_option_def OclIsTypeOf\<^sub>P\<^sub>e\<^sub>r\<^sub>s\<^sub>o\<^sub>n_Galaxy OclIsTypeOf\<^sub>P\<^sub>l\<^sub>a\<^sub>n\<^sub>e\<^sub>t_Galaxy split: option.split ty\<E>\<X>\<T>\<^sub>G\<^sub>a\<^sub>l\<^sub>a\<^sub>x\<^sub>y.split ty\<^sub>G\<^sub>a\<^sub>l\<^sub>a\<^sub>x\<^sub>y.split ty\<E>\<X>\<T>\<^sub>P\<^sub>e\<^sub>r\<^sub>s\<^sub>o\<^sub>n.split ty\<^sub>P\<^sub>e\<^sub>r\<^sub>s\<^sub>o\<^sub>n.split ty\<E>\<X>\<T>\<^sub>P\<^sub>l\<^sub>a\<^sub>n\<^sub>e\<^sub>t.split ty\<^sub>P\<^sub>l\<^sub>a\<^sub>n\<^sub>e\<^sub>t.split)
 by((simp_all add: false_def true_def OclOr_def OclAnd_def OclNot_def)?) 
 lemma actual_eq_static\<^sub>O\<^sub>c\<^sub>l\<^sub>A\<^sub>n\<^sub>y : 
 assumes isdef: "\<tau> \<Turnstile> (\<delta> (X))"
 shows "\<tau> \<Turnstile> ((X::OclAny) .oclIsKindOf(OclAny))"
   apply(simp only: OclValid_def, insert isdef)
   apply(simp only: OclIsKindOf\<^sub>O\<^sub>c\<^sub>l\<^sub>A\<^sub>n\<^sub>y_OclAny, subst (1) cp_OclOr, simp only: OclIsKindOf\<^sub>G\<^sub>a\<^sub>l\<^sub>a\<^sub>x\<^sub>y_OclAny, subst (2 1) cp_OclOr, simp only: OclIsKindOf\<^sub>P\<^sub>l\<^sub>a\<^sub>n\<^sub>e\<^sub>t_OclAny, subst (3 2 1) cp_OclOr, simp only: OclIsKindOf\<^sub>P\<^sub>e\<^sub>r\<^sub>s\<^sub>o\<^sub>n_OclAny)
-  apply(auto simp: cp_OclOr[symmetric ] foundation16 bot_option_def OclIsTypeOf\<^sub>P\<^sub>e\<^sub>r\<^sub>s\<^sub>o\<^sub>n_OclAny OclIsTypeOf\<^sub>P\<^sub>l\<^sub>a\<^sub>n\<^sub>e\<^sub>t_OclAny OclIsTypeOf\<^sub>G\<^sub>a\<^sub>l\<^sub>a\<^sub>x\<^sub>y_OclAny split: option.split type\<^sub>O\<^sub>c\<^sub>l\<^sub>A\<^sub>n\<^sub>y.split typeoid\<^sub>O\<^sub>c\<^sub>l\<^sub>A\<^sub>n\<^sub>y.split type\<^sub>P\<^sub>e\<^sub>r\<^sub>s\<^sub>o\<^sub>n.split typeoid\<^sub>P\<^sub>e\<^sub>r\<^sub>s\<^sub>o\<^sub>n.split type\<^sub>P\<^sub>l\<^sub>a\<^sub>n\<^sub>e\<^sub>t.split typeoid\<^sub>P\<^sub>l\<^sub>a\<^sub>n\<^sub>e\<^sub>t.split type\<^sub>G\<^sub>a\<^sub>l\<^sub>a\<^sub>x\<^sub>y.split typeoid\<^sub>G\<^sub>a\<^sub>l\<^sub>a\<^sub>x\<^sub>y.split)
+  apply(auto simp: cp_OclOr[symmetric ] foundation16 bot_option_def OclIsTypeOf\<^sub>P\<^sub>e\<^sub>r\<^sub>s\<^sub>o\<^sub>n_OclAny OclIsTypeOf\<^sub>P\<^sub>l\<^sub>a\<^sub>n\<^sub>e\<^sub>t_OclAny OclIsTypeOf\<^sub>G\<^sub>a\<^sub>l\<^sub>a\<^sub>x\<^sub>y_OclAny split: option.split ty\<E>\<X>\<T>\<^sub>O\<^sub>c\<^sub>l\<^sub>A\<^sub>n\<^sub>y.split ty\<^sub>O\<^sub>c\<^sub>l\<^sub>A\<^sub>n\<^sub>y.split ty\<E>\<X>\<T>\<^sub>P\<^sub>e\<^sub>r\<^sub>s\<^sub>o\<^sub>n.split ty\<^sub>P\<^sub>e\<^sub>r\<^sub>s\<^sub>o\<^sub>n.split ty\<E>\<X>\<T>\<^sub>P\<^sub>l\<^sub>a\<^sub>n\<^sub>e\<^sub>t.split ty\<^sub>P\<^sub>l\<^sub>a\<^sub>n\<^sub>e\<^sub>t.split ty\<E>\<X>\<T>\<^sub>G\<^sub>a\<^sub>l\<^sub>a\<^sub>x\<^sub>y.split ty\<^sub>G\<^sub>a\<^sub>l\<^sub>a\<^sub>x\<^sub>y.split)
 by((simp_all add: false_def true_def OclOr_def OclAnd_def OclNot_def)?) 
 
 (* 82 ************************************ 546 + 6 *)
@@ -2392,7 +2392,7 @@ lemma Planet_OclAllInstances_generic_OclIsTypeOf\<^sub>P\<^sub>l\<^sub>a\<^sub>n
 assumes [simp]: "(\<And>x. (pre_post ((x , x))) = x)"
 shows "(\<exists>\<tau>. \<tau> \<Turnstile> (not ((UML_Set.OclForall ((OclAllInstances_generic (pre_post) (Planet))) (OclIsTypeOf\<^sub>P\<^sub>l\<^sub>a\<^sub>n\<^sub>e\<^sub>t)))))"
   proof - fix oid a show ?thesis
-  proof - let ?t0 = "(state.make ((Map.empty (oid \<mapsto> (in\<^sub>P\<^sub>l\<^sub>a\<^sub>n\<^sub>e\<^sub>t ((mkoid\<^sub>P\<^sub>l\<^sub>a\<^sub>n\<^sub>e\<^sub>t ((mk\<^sub>P\<^sub>l\<^sub>a\<^sub>n\<^sub>e\<^sub>t_\<^sub>P\<^sub>e\<^sub>r\<^sub>s\<^sub>o\<^sub>n (a))) (None) (None))))))) (Map.empty))" show ?thesis
+  proof - let ?t0 = "(state.make ((Map.empty (oid \<mapsto> (in\<^sub>P\<^sub>l\<^sub>a\<^sub>n\<^sub>e\<^sub>t ((mk\<^sub>P\<^sub>l\<^sub>a\<^sub>n\<^sub>e\<^sub>t ((mk\<E>\<X>\<T>\<^sub>P\<^sub>l\<^sub>a\<^sub>n\<^sub>e\<^sub>t_\<^sub>P\<^sub>e\<^sub>r\<^sub>s\<^sub>o\<^sub>n (a))) (None) (None))))))) (Map.empty))" show ?thesis
   apply(rule exI[where x = "(?t0 , ?t0)"], simp add: OclValid_def del: OclAllInstances_generic_def)
   apply(simp only: UML_Set.OclForall_def refl if_True OclAllInstances_generic_defined[simplified OclValid_def])
   apply(simp only: OclAllInstances_generic_def OclAsType\<^sub>P\<^sub>l\<^sub>a\<^sub>n\<^sub>e\<^sub>t_\<AA>_def)
@@ -2426,7 +2426,7 @@ lemma Galaxy_OclAllInstances_generic_OclIsTypeOf\<^sub>G\<^sub>a\<^sub>l\<^sub>a
 assumes [simp]: "(\<And>x. (pre_post ((x , x))) = x)"
 shows "(\<exists>\<tau>. \<tau> \<Turnstile> (not ((UML_Set.OclForall ((OclAllInstances_generic (pre_post) (Galaxy))) (OclIsTypeOf\<^sub>G\<^sub>a\<^sub>l\<^sub>a\<^sub>x\<^sub>y)))))"
   proof - fix oid a show ?thesis
-  proof - let ?t0 = "(state.make ((Map.empty (oid \<mapsto> (in\<^sub>G\<^sub>a\<^sub>l\<^sub>a\<^sub>x\<^sub>y ((mkoid\<^sub>G\<^sub>a\<^sub>l\<^sub>a\<^sub>x\<^sub>y ((mk\<^sub>G\<^sub>a\<^sub>l\<^sub>a\<^sub>x\<^sub>y_\<^sub>P\<^sub>l\<^sub>a\<^sub>n\<^sub>e\<^sub>t (a))) (None) (None) (None))))))) (Map.empty))" show ?thesis
+  proof - let ?t0 = "(state.make ((Map.empty (oid \<mapsto> (in\<^sub>G\<^sub>a\<^sub>l\<^sub>a\<^sub>x\<^sub>y ((mk\<^sub>G\<^sub>a\<^sub>l\<^sub>a\<^sub>x\<^sub>y ((mk\<E>\<X>\<T>\<^sub>G\<^sub>a\<^sub>l\<^sub>a\<^sub>x\<^sub>y_\<^sub>P\<^sub>l\<^sub>a\<^sub>n\<^sub>e\<^sub>t (a))) (None) (None) (None))))))) (Map.empty))" show ?thesis
   apply(rule exI[where x = "(?t0 , ?t0)"], simp add: OclValid_def del: OclAllInstances_generic_def)
   apply(simp only: UML_Set.OclForall_def refl if_True OclAllInstances_generic_defined[simplified OclValid_def])
   apply(simp only: OclAllInstances_generic_def OclAsType\<^sub>G\<^sub>a\<^sub>l\<^sub>a\<^sub>x\<^sub>y_\<AA>_def)
@@ -2460,7 +2460,7 @@ lemma OclAny_OclAllInstances_generic_OclIsTypeOf\<^sub>O\<^sub>c\<^sub>l\<^sub>A
 assumes [simp]: "(\<And>x. (pre_post ((x , x))) = x)"
 shows "(\<exists>\<tau>. \<tau> \<Turnstile> (not ((UML_Set.OclForall ((OclAllInstances_generic (pre_post) (OclAny))) (OclIsTypeOf\<^sub>O\<^sub>c\<^sub>l\<^sub>A\<^sub>n\<^sub>y)))))"
   proof - fix oid a show ?thesis
-  proof - let ?t0 = "(state.make ((Map.empty (oid \<mapsto> (in\<^sub>O\<^sub>c\<^sub>l\<^sub>A\<^sub>n\<^sub>y ((mkoid\<^sub>O\<^sub>c\<^sub>l\<^sub>A\<^sub>n\<^sub>y ((mk\<^sub>O\<^sub>c\<^sub>l\<^sub>A\<^sub>n\<^sub>y_\<^sub>G\<^sub>a\<^sub>l\<^sub>a\<^sub>x\<^sub>y (a))))))))) (Map.empty))" show ?thesis
+  proof - let ?t0 = "(state.make ((Map.empty (oid \<mapsto> (in\<^sub>O\<^sub>c\<^sub>l\<^sub>A\<^sub>n\<^sub>y ((mk\<^sub>O\<^sub>c\<^sub>l\<^sub>A\<^sub>n\<^sub>y ((mk\<E>\<X>\<T>\<^sub>O\<^sub>c\<^sub>l\<^sub>A\<^sub>n\<^sub>y_\<^sub>G\<^sub>a\<^sub>l\<^sub>a\<^sub>x\<^sub>y (a))))))))) (Map.empty))" show ?thesis
   apply(rule exI[where x = "(?t0 , ?t0)"], simp add: OclValid_def del: OclAllInstances_generic_def)
   apply(simp only: UML_Set.OclForall_def refl if_True OclAllInstances_generic_defined[simplified OclValid_def])
   apply(simp only: OclAllInstances_generic_def OclAsType\<^sub>O\<^sub>c\<^sub>l\<^sub>A\<^sub>n\<^sub>y_\<AA>_def)
@@ -2715,39 +2715,39 @@ text{*
    pointer undefined in state or not referencing a type conform object representation  *}
 
 (* 113 ************************************ 664 + 15 *)
-definition "select\<^sub>P\<^sub>e\<^sub>r\<^sub>s\<^sub>o\<^sub>n\<B>\<O>\<S>\<S> f = (\<lambda> (mkoid\<^sub>P\<^sub>e\<^sub>r\<^sub>s\<^sub>o\<^sub>n (_) (\<bottom>) (_)) \<Rightarrow> null
-    | (mkoid\<^sub>P\<^sub>e\<^sub>r\<^sub>s\<^sub>o\<^sub>n (_) (\<lfloor>\<B>\<O>\<S>\<S>\<rfloor>) (_)) \<Rightarrow> (f (\<B>\<O>\<S>\<S>)))"
-definition "select\<^sub>P\<^sub>e\<^sub>r\<^sub>s\<^sub>o\<^sub>n\<S>\<A>\<L>\<A>\<R>\<Y> f = (\<lambda> (mkoid\<^sub>P\<^sub>e\<^sub>r\<^sub>s\<^sub>o\<^sub>n (_) (_) (\<bottom>)) \<Rightarrow> null
-    | (mkoid\<^sub>P\<^sub>e\<^sub>r\<^sub>s\<^sub>o\<^sub>n (_) (_) (\<lfloor>\<S>\<A>\<L>\<A>\<R>\<Y>\<rfloor>)) \<Rightarrow> (f (\<S>\<A>\<L>\<A>\<R>\<Y>)))"
-definition "select\<^sub>P\<^sub>l\<^sub>a\<^sub>n\<^sub>e\<^sub>t\<W>\<O>\<R>\<M>\<H>\<O>\<L>\<E> f = (\<lambda> (mkoid\<^sub>P\<^sub>l\<^sub>a\<^sub>n\<^sub>e\<^sub>t (_) (\<bottom>) (_)) \<Rightarrow> null
-    | (mkoid\<^sub>P\<^sub>l\<^sub>a\<^sub>n\<^sub>e\<^sub>t (_) (\<lfloor>\<W>\<O>\<R>\<M>\<H>\<O>\<L>\<E>\<rfloor>) (_)) \<Rightarrow> (f (\<W>\<O>\<R>\<M>\<H>\<O>\<L>\<E>)))"
-definition "select\<^sub>P\<^sub>l\<^sub>a\<^sub>n\<^sub>e\<^sub>t\<W>\<E>\<I>\<G>\<H>\<T> f = (\<lambda> (mkoid\<^sub>P\<^sub>l\<^sub>a\<^sub>n\<^sub>e\<^sub>t (_) (_) (\<bottom>)) \<Rightarrow> null
-    | (mkoid\<^sub>P\<^sub>l\<^sub>a\<^sub>n\<^sub>e\<^sub>t (_) (_) (\<lfloor>\<W>\<E>\<I>\<G>\<H>\<T>\<rfloor>)) \<Rightarrow> (f (\<W>\<E>\<I>\<G>\<H>\<T>)))"
-definition "select\<^sub>G\<^sub>a\<^sub>l\<^sub>a\<^sub>x\<^sub>y\<S>\<O>\<U>\<N>\<D> f = (\<lambda> (mkoid\<^sub>G\<^sub>a\<^sub>l\<^sub>a\<^sub>x\<^sub>y (_) (\<bottom>) (_) (_)) \<Rightarrow> null
-    | (mkoid\<^sub>G\<^sub>a\<^sub>l\<^sub>a\<^sub>x\<^sub>y (_) (\<lfloor>\<S>\<O>\<U>\<N>\<D>\<rfloor>) (_) (_)) \<Rightarrow> (f (\<S>\<O>\<U>\<N>\<D>)))"
-definition "select\<^sub>G\<^sub>a\<^sub>l\<^sub>a\<^sub>x\<^sub>y\<M>\<O>\<V>\<I>\<N>\<G> f = (\<lambda> (mkoid\<^sub>G\<^sub>a\<^sub>l\<^sub>a\<^sub>x\<^sub>y (_) (_) (\<bottom>) (_)) \<Rightarrow> null
-    | (mkoid\<^sub>G\<^sub>a\<^sub>l\<^sub>a\<^sub>x\<^sub>y (_) (_) (\<lfloor>\<M>\<O>\<V>\<I>\<N>\<G>\<rfloor>) (_)) \<Rightarrow> (f (\<M>\<O>\<V>\<I>\<N>\<G>)))"
-definition "select\<^sub>G\<^sub>a\<^sub>l\<^sub>a\<^sub>x\<^sub>y\<O>\<U>\<T>\<E>\<R>095\<W>\<O>\<R>\<L>\<D> f = (\<lambda> (mkoid\<^sub>G\<^sub>a\<^sub>l\<^sub>a\<^sub>x\<^sub>y (_) (_) (_) (\<bottom>)) \<Rightarrow> null
-    | (mkoid\<^sub>G\<^sub>a\<^sub>l\<^sub>a\<^sub>x\<^sub>y (_) (_) (_) (\<lfloor>\<O>\<U>\<T>\<E>\<R>095\<W>\<O>\<R>\<L>\<D>\<rfloor>)) \<Rightarrow> (f (\<O>\<U>\<T>\<E>\<R>095\<W>\<O>\<R>\<L>\<D>)))"
-definition "select\<^sub>P\<^sub>e\<^sub>r\<^sub>s\<^sub>o\<^sub>n\<W>\<O>\<R>\<M>\<H>\<O>\<L>\<E> f = (\<lambda> (mkoid\<^sub>P\<^sub>e\<^sub>r\<^sub>s\<^sub>o\<^sub>n ((mk\<^sub>P\<^sub>e\<^sub>r\<^sub>s\<^sub>o\<^sub>n (_) (\<bottom>) (_) (_) (_) (_))) (_) (_)) \<Rightarrow> null
-    | (mkoid\<^sub>P\<^sub>e\<^sub>r\<^sub>s\<^sub>o\<^sub>n ((mk\<^sub>P\<^sub>e\<^sub>r\<^sub>s\<^sub>o\<^sub>n (_) (\<lfloor>\<W>\<O>\<R>\<M>\<H>\<O>\<L>\<E>\<rfloor>) (_) (_) (_) (_))) (_) (_)) \<Rightarrow> (f (\<W>\<O>\<R>\<M>\<H>\<O>\<L>\<E>)))"
-definition "select\<^sub>P\<^sub>e\<^sub>r\<^sub>s\<^sub>o\<^sub>n\<W>\<E>\<I>\<G>\<H>\<T> f = (\<lambda> (mkoid\<^sub>P\<^sub>e\<^sub>r\<^sub>s\<^sub>o\<^sub>n ((mk\<^sub>P\<^sub>e\<^sub>r\<^sub>s\<^sub>o\<^sub>n (_) (_) (\<bottom>) (_) (_) (_))) (_) (_)) \<Rightarrow> null
-    | (mkoid\<^sub>P\<^sub>e\<^sub>r\<^sub>s\<^sub>o\<^sub>n ((mk\<^sub>P\<^sub>e\<^sub>r\<^sub>s\<^sub>o\<^sub>n (_) (_) (\<lfloor>\<W>\<E>\<I>\<G>\<H>\<T>\<rfloor>) (_) (_) (_))) (_) (_)) \<Rightarrow> (f (\<W>\<E>\<I>\<G>\<H>\<T>)))"
-definition "select\<^sub>P\<^sub>e\<^sub>r\<^sub>s\<^sub>o\<^sub>n\<S>\<O>\<U>\<N>\<D> f = (\<lambda> (mkoid\<^sub>P\<^sub>e\<^sub>r\<^sub>s\<^sub>o\<^sub>n ((mk\<^sub>P\<^sub>e\<^sub>r\<^sub>s\<^sub>o\<^sub>n (_) (_) (_) (\<bottom>) (_) (_))) (_) (_)) \<Rightarrow> null
-    | (mkoid\<^sub>P\<^sub>e\<^sub>r\<^sub>s\<^sub>o\<^sub>n ((mk\<^sub>P\<^sub>e\<^sub>r\<^sub>s\<^sub>o\<^sub>n (_) (_) (_) (\<lfloor>\<S>\<O>\<U>\<N>\<D>\<rfloor>) (_) (_))) (_) (_)) \<Rightarrow> (f (\<S>\<O>\<U>\<N>\<D>)))"
-definition "select\<^sub>P\<^sub>e\<^sub>r\<^sub>s\<^sub>o\<^sub>n\<M>\<O>\<V>\<I>\<N>\<G> f = (\<lambda> (mkoid\<^sub>P\<^sub>e\<^sub>r\<^sub>s\<^sub>o\<^sub>n ((mk\<^sub>P\<^sub>e\<^sub>r\<^sub>s\<^sub>o\<^sub>n (_) (_) (_) (_) (\<bottom>) (_))) (_) (_)) \<Rightarrow> null
-    | (mkoid\<^sub>P\<^sub>e\<^sub>r\<^sub>s\<^sub>o\<^sub>n ((mk\<^sub>P\<^sub>e\<^sub>r\<^sub>s\<^sub>o\<^sub>n (_) (_) (_) (_) (\<lfloor>\<M>\<O>\<V>\<I>\<N>\<G>\<rfloor>) (_))) (_) (_)) \<Rightarrow> (f (\<M>\<O>\<V>\<I>\<N>\<G>)))"
-definition "select\<^sub>P\<^sub>e\<^sub>r\<^sub>s\<^sub>o\<^sub>n\<O>\<U>\<T>\<E>\<R>095\<W>\<O>\<R>\<L>\<D> f = (\<lambda> (mkoid\<^sub>P\<^sub>e\<^sub>r\<^sub>s\<^sub>o\<^sub>n ((mk\<^sub>P\<^sub>e\<^sub>r\<^sub>s\<^sub>o\<^sub>n (_) (_) (_) (_) (_) (\<bottom>))) (_) (_)) \<Rightarrow> null
-    | (mkoid\<^sub>P\<^sub>e\<^sub>r\<^sub>s\<^sub>o\<^sub>n ((mk\<^sub>P\<^sub>e\<^sub>r\<^sub>s\<^sub>o\<^sub>n (_) (_) (_) (_) (_) (\<lfloor>\<O>\<U>\<T>\<E>\<R>095\<W>\<O>\<R>\<L>\<D>\<rfloor>))) (_) (_)) \<Rightarrow> (f (\<O>\<U>\<T>\<E>\<R>095\<W>\<O>\<R>\<L>\<D>)))"
-definition "select\<^sub>P\<^sub>l\<^sub>a\<^sub>n\<^sub>e\<^sub>t\<S>\<O>\<U>\<N>\<D> f = (\<lambda> (mkoid\<^sub>P\<^sub>l\<^sub>a\<^sub>n\<^sub>e\<^sub>t ((mk\<^sub>P\<^sub>l\<^sub>a\<^sub>n\<^sub>e\<^sub>t (_) (\<bottom>) (_) (_))) (_) (_)) \<Rightarrow> null
-    | (mkoid\<^sub>P\<^sub>l\<^sub>a\<^sub>n\<^sub>e\<^sub>t ((mk\<^sub>P\<^sub>l\<^sub>a\<^sub>n\<^sub>e\<^sub>t (_) (\<lfloor>\<S>\<O>\<U>\<N>\<D>\<rfloor>) (_) (_))) (_) (_)) \<Rightarrow> (f (\<S>\<O>\<U>\<N>\<D>))
-    | (mkoid\<^sub>P\<^sub>l\<^sub>a\<^sub>n\<^sub>e\<^sub>t ((mk\<^sub>P\<^sub>l\<^sub>a\<^sub>n\<^sub>e\<^sub>t_\<^sub>P\<^sub>e\<^sub>r\<^sub>s\<^sub>o\<^sub>n (person))) (_) (_)) \<Rightarrow> (select\<^sub>P\<^sub>e\<^sub>r\<^sub>s\<^sub>o\<^sub>n\<S>\<O>\<U>\<N>\<D> (f) (person)))"
-definition "select\<^sub>P\<^sub>l\<^sub>a\<^sub>n\<^sub>e\<^sub>t\<M>\<O>\<V>\<I>\<N>\<G> f = (\<lambda> (mkoid\<^sub>P\<^sub>l\<^sub>a\<^sub>n\<^sub>e\<^sub>t ((mk\<^sub>P\<^sub>l\<^sub>a\<^sub>n\<^sub>e\<^sub>t (_) (_) (\<bottom>) (_))) (_) (_)) \<Rightarrow> null
-    | (mkoid\<^sub>P\<^sub>l\<^sub>a\<^sub>n\<^sub>e\<^sub>t ((mk\<^sub>P\<^sub>l\<^sub>a\<^sub>n\<^sub>e\<^sub>t (_) (_) (\<lfloor>\<M>\<O>\<V>\<I>\<N>\<G>\<rfloor>) (_))) (_) (_)) \<Rightarrow> (f (\<M>\<O>\<V>\<I>\<N>\<G>))
-    | (mkoid\<^sub>P\<^sub>l\<^sub>a\<^sub>n\<^sub>e\<^sub>t ((mk\<^sub>P\<^sub>l\<^sub>a\<^sub>n\<^sub>e\<^sub>t_\<^sub>P\<^sub>e\<^sub>r\<^sub>s\<^sub>o\<^sub>n (person))) (_) (_)) \<Rightarrow> (select\<^sub>P\<^sub>e\<^sub>r\<^sub>s\<^sub>o\<^sub>n\<M>\<O>\<V>\<I>\<N>\<G> (f) (person)))"
-definition "select\<^sub>P\<^sub>l\<^sub>a\<^sub>n\<^sub>e\<^sub>t\<O>\<U>\<T>\<E>\<R>095\<W>\<O>\<R>\<L>\<D> f = (\<lambda> (mkoid\<^sub>P\<^sub>l\<^sub>a\<^sub>n\<^sub>e\<^sub>t ((mk\<^sub>P\<^sub>l\<^sub>a\<^sub>n\<^sub>e\<^sub>t (_) (_) (_) (\<bottom>))) (_) (_)) \<Rightarrow> null
-    | (mkoid\<^sub>P\<^sub>l\<^sub>a\<^sub>n\<^sub>e\<^sub>t ((mk\<^sub>P\<^sub>l\<^sub>a\<^sub>n\<^sub>e\<^sub>t (_) (_) (_) (\<lfloor>\<O>\<U>\<T>\<E>\<R>095\<W>\<O>\<R>\<L>\<D>\<rfloor>))) (_) (_)) \<Rightarrow> (f (\<O>\<U>\<T>\<E>\<R>095\<W>\<O>\<R>\<L>\<D>))
-    | (mkoid\<^sub>P\<^sub>l\<^sub>a\<^sub>n\<^sub>e\<^sub>t ((mk\<^sub>P\<^sub>l\<^sub>a\<^sub>n\<^sub>e\<^sub>t_\<^sub>P\<^sub>e\<^sub>r\<^sub>s\<^sub>o\<^sub>n (person))) (_) (_)) \<Rightarrow> (select\<^sub>P\<^sub>e\<^sub>r\<^sub>s\<^sub>o\<^sub>n\<O>\<U>\<T>\<E>\<R>095\<W>\<O>\<R>\<L>\<D> (f) (person)))"
+definition "select\<^sub>P\<^sub>e\<^sub>r\<^sub>s\<^sub>o\<^sub>n\<B>\<O>\<S>\<S> f = (\<lambda> (mk\<^sub>P\<^sub>e\<^sub>r\<^sub>s\<^sub>o\<^sub>n (_) (\<bottom>) (_)) \<Rightarrow> null
+    | (mk\<^sub>P\<^sub>e\<^sub>r\<^sub>s\<^sub>o\<^sub>n (_) (\<lfloor>\<B>\<O>\<S>\<S>\<rfloor>) (_)) \<Rightarrow> (f (\<B>\<O>\<S>\<S>)))"
+definition "select\<^sub>P\<^sub>e\<^sub>r\<^sub>s\<^sub>o\<^sub>n\<S>\<A>\<L>\<A>\<R>\<Y> f = (\<lambda> (mk\<^sub>P\<^sub>e\<^sub>r\<^sub>s\<^sub>o\<^sub>n (_) (_) (\<bottom>)) \<Rightarrow> null
+    | (mk\<^sub>P\<^sub>e\<^sub>r\<^sub>s\<^sub>o\<^sub>n (_) (_) (\<lfloor>\<S>\<A>\<L>\<A>\<R>\<Y>\<rfloor>)) \<Rightarrow> (f (\<S>\<A>\<L>\<A>\<R>\<Y>)))"
+definition "select\<^sub>P\<^sub>l\<^sub>a\<^sub>n\<^sub>e\<^sub>t\<W>\<O>\<R>\<M>\<H>\<O>\<L>\<E> f = (\<lambda> (mk\<^sub>P\<^sub>l\<^sub>a\<^sub>n\<^sub>e\<^sub>t (_) (\<bottom>) (_)) \<Rightarrow> null
+    | (mk\<^sub>P\<^sub>l\<^sub>a\<^sub>n\<^sub>e\<^sub>t (_) (\<lfloor>\<W>\<O>\<R>\<M>\<H>\<O>\<L>\<E>\<rfloor>) (_)) \<Rightarrow> (f (\<W>\<O>\<R>\<M>\<H>\<O>\<L>\<E>)))"
+definition "select\<^sub>P\<^sub>l\<^sub>a\<^sub>n\<^sub>e\<^sub>t\<W>\<E>\<I>\<G>\<H>\<T> f = (\<lambda> (mk\<^sub>P\<^sub>l\<^sub>a\<^sub>n\<^sub>e\<^sub>t (_) (_) (\<bottom>)) \<Rightarrow> null
+    | (mk\<^sub>P\<^sub>l\<^sub>a\<^sub>n\<^sub>e\<^sub>t (_) (_) (\<lfloor>\<W>\<E>\<I>\<G>\<H>\<T>\<rfloor>)) \<Rightarrow> (f (\<W>\<E>\<I>\<G>\<H>\<T>)))"
+definition "select\<^sub>G\<^sub>a\<^sub>l\<^sub>a\<^sub>x\<^sub>y\<S>\<O>\<U>\<N>\<D> f = (\<lambda> (mk\<^sub>G\<^sub>a\<^sub>l\<^sub>a\<^sub>x\<^sub>y (_) (\<bottom>) (_) (_)) \<Rightarrow> null
+    | (mk\<^sub>G\<^sub>a\<^sub>l\<^sub>a\<^sub>x\<^sub>y (_) (\<lfloor>\<S>\<O>\<U>\<N>\<D>\<rfloor>) (_) (_)) \<Rightarrow> (f (\<S>\<O>\<U>\<N>\<D>)))"
+definition "select\<^sub>G\<^sub>a\<^sub>l\<^sub>a\<^sub>x\<^sub>y\<M>\<O>\<V>\<I>\<N>\<G> f = (\<lambda> (mk\<^sub>G\<^sub>a\<^sub>l\<^sub>a\<^sub>x\<^sub>y (_) (_) (\<bottom>) (_)) \<Rightarrow> null
+    | (mk\<^sub>G\<^sub>a\<^sub>l\<^sub>a\<^sub>x\<^sub>y (_) (_) (\<lfloor>\<M>\<O>\<V>\<I>\<N>\<G>\<rfloor>) (_)) \<Rightarrow> (f (\<M>\<O>\<V>\<I>\<N>\<G>)))"
+definition "select\<^sub>G\<^sub>a\<^sub>l\<^sub>a\<^sub>x\<^sub>y\<O>\<U>\<T>\<E>\<R>095\<W>\<O>\<R>\<L>\<D> f = (\<lambda> (mk\<^sub>G\<^sub>a\<^sub>l\<^sub>a\<^sub>x\<^sub>y (_) (_) (_) (\<bottom>)) \<Rightarrow> null
+    | (mk\<^sub>G\<^sub>a\<^sub>l\<^sub>a\<^sub>x\<^sub>y (_) (_) (_) (\<lfloor>\<O>\<U>\<T>\<E>\<R>095\<W>\<O>\<R>\<L>\<D>\<rfloor>)) \<Rightarrow> (f (\<O>\<U>\<T>\<E>\<R>095\<W>\<O>\<R>\<L>\<D>)))"
+definition "select\<^sub>P\<^sub>e\<^sub>r\<^sub>s\<^sub>o\<^sub>n\<W>\<O>\<R>\<M>\<H>\<O>\<L>\<E> f = (\<lambda> (mk\<^sub>P\<^sub>e\<^sub>r\<^sub>s\<^sub>o\<^sub>n ((mk\<E>\<X>\<T>\<^sub>P\<^sub>e\<^sub>r\<^sub>s\<^sub>o\<^sub>n (_) (\<bottom>) (_) (_) (_) (_))) (_) (_)) \<Rightarrow> null
+    | (mk\<^sub>P\<^sub>e\<^sub>r\<^sub>s\<^sub>o\<^sub>n ((mk\<E>\<X>\<T>\<^sub>P\<^sub>e\<^sub>r\<^sub>s\<^sub>o\<^sub>n (_) (\<lfloor>\<W>\<O>\<R>\<M>\<H>\<O>\<L>\<E>\<rfloor>) (_) (_) (_) (_))) (_) (_)) \<Rightarrow> (f (\<W>\<O>\<R>\<M>\<H>\<O>\<L>\<E>)))"
+definition "select\<^sub>P\<^sub>e\<^sub>r\<^sub>s\<^sub>o\<^sub>n\<W>\<E>\<I>\<G>\<H>\<T> f = (\<lambda> (mk\<^sub>P\<^sub>e\<^sub>r\<^sub>s\<^sub>o\<^sub>n ((mk\<E>\<X>\<T>\<^sub>P\<^sub>e\<^sub>r\<^sub>s\<^sub>o\<^sub>n (_) (_) (\<bottom>) (_) (_) (_))) (_) (_)) \<Rightarrow> null
+    | (mk\<^sub>P\<^sub>e\<^sub>r\<^sub>s\<^sub>o\<^sub>n ((mk\<E>\<X>\<T>\<^sub>P\<^sub>e\<^sub>r\<^sub>s\<^sub>o\<^sub>n (_) (_) (\<lfloor>\<W>\<E>\<I>\<G>\<H>\<T>\<rfloor>) (_) (_) (_))) (_) (_)) \<Rightarrow> (f (\<W>\<E>\<I>\<G>\<H>\<T>)))"
+definition "select\<^sub>P\<^sub>e\<^sub>r\<^sub>s\<^sub>o\<^sub>n\<S>\<O>\<U>\<N>\<D> f = (\<lambda> (mk\<^sub>P\<^sub>e\<^sub>r\<^sub>s\<^sub>o\<^sub>n ((mk\<E>\<X>\<T>\<^sub>P\<^sub>e\<^sub>r\<^sub>s\<^sub>o\<^sub>n (_) (_) (_) (\<bottom>) (_) (_))) (_) (_)) \<Rightarrow> null
+    | (mk\<^sub>P\<^sub>e\<^sub>r\<^sub>s\<^sub>o\<^sub>n ((mk\<E>\<X>\<T>\<^sub>P\<^sub>e\<^sub>r\<^sub>s\<^sub>o\<^sub>n (_) (_) (_) (\<lfloor>\<S>\<O>\<U>\<N>\<D>\<rfloor>) (_) (_))) (_) (_)) \<Rightarrow> (f (\<S>\<O>\<U>\<N>\<D>)))"
+definition "select\<^sub>P\<^sub>e\<^sub>r\<^sub>s\<^sub>o\<^sub>n\<M>\<O>\<V>\<I>\<N>\<G> f = (\<lambda> (mk\<^sub>P\<^sub>e\<^sub>r\<^sub>s\<^sub>o\<^sub>n ((mk\<E>\<X>\<T>\<^sub>P\<^sub>e\<^sub>r\<^sub>s\<^sub>o\<^sub>n (_) (_) (_) (_) (\<bottom>) (_))) (_) (_)) \<Rightarrow> null
+    | (mk\<^sub>P\<^sub>e\<^sub>r\<^sub>s\<^sub>o\<^sub>n ((mk\<E>\<X>\<T>\<^sub>P\<^sub>e\<^sub>r\<^sub>s\<^sub>o\<^sub>n (_) (_) (_) (_) (\<lfloor>\<M>\<O>\<V>\<I>\<N>\<G>\<rfloor>) (_))) (_) (_)) \<Rightarrow> (f (\<M>\<O>\<V>\<I>\<N>\<G>)))"
+definition "select\<^sub>P\<^sub>e\<^sub>r\<^sub>s\<^sub>o\<^sub>n\<O>\<U>\<T>\<E>\<R>095\<W>\<O>\<R>\<L>\<D> f = (\<lambda> (mk\<^sub>P\<^sub>e\<^sub>r\<^sub>s\<^sub>o\<^sub>n ((mk\<E>\<X>\<T>\<^sub>P\<^sub>e\<^sub>r\<^sub>s\<^sub>o\<^sub>n (_) (_) (_) (_) (_) (\<bottom>))) (_) (_)) \<Rightarrow> null
+    | (mk\<^sub>P\<^sub>e\<^sub>r\<^sub>s\<^sub>o\<^sub>n ((mk\<E>\<X>\<T>\<^sub>P\<^sub>e\<^sub>r\<^sub>s\<^sub>o\<^sub>n (_) (_) (_) (_) (_) (\<lfloor>\<O>\<U>\<T>\<E>\<R>095\<W>\<O>\<R>\<L>\<D>\<rfloor>))) (_) (_)) \<Rightarrow> (f (\<O>\<U>\<T>\<E>\<R>095\<W>\<O>\<R>\<L>\<D>)))"
+definition "select\<^sub>P\<^sub>l\<^sub>a\<^sub>n\<^sub>e\<^sub>t\<S>\<O>\<U>\<N>\<D> f = (\<lambda> (mk\<^sub>P\<^sub>l\<^sub>a\<^sub>n\<^sub>e\<^sub>t ((mk\<E>\<X>\<T>\<^sub>P\<^sub>l\<^sub>a\<^sub>n\<^sub>e\<^sub>t (_) (\<bottom>) (_) (_))) (_) (_)) \<Rightarrow> null
+    | (mk\<^sub>P\<^sub>l\<^sub>a\<^sub>n\<^sub>e\<^sub>t ((mk\<E>\<X>\<T>\<^sub>P\<^sub>l\<^sub>a\<^sub>n\<^sub>e\<^sub>t (_) (\<lfloor>\<S>\<O>\<U>\<N>\<D>\<rfloor>) (_) (_))) (_) (_)) \<Rightarrow> (f (\<S>\<O>\<U>\<N>\<D>))
+    | (mk\<^sub>P\<^sub>l\<^sub>a\<^sub>n\<^sub>e\<^sub>t ((mk\<E>\<X>\<T>\<^sub>P\<^sub>l\<^sub>a\<^sub>n\<^sub>e\<^sub>t_\<^sub>P\<^sub>e\<^sub>r\<^sub>s\<^sub>o\<^sub>n (person))) (_) (_)) \<Rightarrow> (select\<^sub>P\<^sub>e\<^sub>r\<^sub>s\<^sub>o\<^sub>n\<S>\<O>\<U>\<N>\<D> (f) (person)))"
+definition "select\<^sub>P\<^sub>l\<^sub>a\<^sub>n\<^sub>e\<^sub>t\<M>\<O>\<V>\<I>\<N>\<G> f = (\<lambda> (mk\<^sub>P\<^sub>l\<^sub>a\<^sub>n\<^sub>e\<^sub>t ((mk\<E>\<X>\<T>\<^sub>P\<^sub>l\<^sub>a\<^sub>n\<^sub>e\<^sub>t (_) (_) (\<bottom>) (_))) (_) (_)) \<Rightarrow> null
+    | (mk\<^sub>P\<^sub>l\<^sub>a\<^sub>n\<^sub>e\<^sub>t ((mk\<E>\<X>\<T>\<^sub>P\<^sub>l\<^sub>a\<^sub>n\<^sub>e\<^sub>t (_) (_) (\<lfloor>\<M>\<O>\<V>\<I>\<N>\<G>\<rfloor>) (_))) (_) (_)) \<Rightarrow> (f (\<M>\<O>\<V>\<I>\<N>\<G>))
+    | (mk\<^sub>P\<^sub>l\<^sub>a\<^sub>n\<^sub>e\<^sub>t ((mk\<E>\<X>\<T>\<^sub>P\<^sub>l\<^sub>a\<^sub>n\<^sub>e\<^sub>t_\<^sub>P\<^sub>e\<^sub>r\<^sub>s\<^sub>o\<^sub>n (person))) (_) (_)) \<Rightarrow> (select\<^sub>P\<^sub>e\<^sub>r\<^sub>s\<^sub>o\<^sub>n\<M>\<O>\<V>\<I>\<N>\<G> (f) (person)))"
+definition "select\<^sub>P\<^sub>l\<^sub>a\<^sub>n\<^sub>e\<^sub>t\<O>\<U>\<T>\<E>\<R>095\<W>\<O>\<R>\<L>\<D> f = (\<lambda> (mk\<^sub>P\<^sub>l\<^sub>a\<^sub>n\<^sub>e\<^sub>t ((mk\<E>\<X>\<T>\<^sub>P\<^sub>l\<^sub>a\<^sub>n\<^sub>e\<^sub>t (_) (_) (_) (\<bottom>))) (_) (_)) \<Rightarrow> null
+    | (mk\<^sub>P\<^sub>l\<^sub>a\<^sub>n\<^sub>e\<^sub>t ((mk\<E>\<X>\<T>\<^sub>P\<^sub>l\<^sub>a\<^sub>n\<^sub>e\<^sub>t (_) (_) (_) (\<lfloor>\<O>\<U>\<T>\<E>\<R>095\<W>\<O>\<R>\<L>\<D>\<rfloor>))) (_) (_)) \<Rightarrow> (f (\<O>\<U>\<T>\<E>\<R>095\<W>\<O>\<R>\<L>\<D>))
+    | (mk\<^sub>P\<^sub>l\<^sub>a\<^sub>n\<^sub>e\<^sub>t ((mk\<E>\<X>\<T>\<^sub>P\<^sub>l\<^sub>a\<^sub>n\<^sub>e\<^sub>t_\<^sub>P\<^sub>e\<^sub>r\<^sub>s\<^sub>o\<^sub>n (person))) (_) (_)) \<Rightarrow> (select\<^sub>P\<^sub>e\<^sub>r\<^sub>s\<^sub>o\<^sub>n\<O>\<U>\<T>\<E>\<R>095\<W>\<O>\<R>\<L>\<D> (f) (person)))"
 
 (* 114 ************************************ 679 + 0 *)
 
@@ -3307,17 +3307,17 @@ definition "inst_assoc1 = (\<lambda>oid_class to_from oid. ((case (deref_assocs_
     | l \<Rightarrow> (Some (l)))::oid list option))"
 
 (* 133 ************************************ 868 + 22 *)
-definition "X\<^sub>P\<^sub>e\<^sub>r\<^sub>s\<^sub>o\<^sub>n1\<^sub>P\<^sub>e\<^sub>r\<^sub>s\<^sub>o\<^sub>n inst_assoc = (mkoid\<^sub>P\<^sub>e\<^sub>r\<^sub>s\<^sub>o\<^sub>n ((mk\<^sub>P\<^sub>e\<^sub>r\<^sub>s\<^sub>o\<^sub>n (oid1) (None) (None) (None) (None) (None))) (((inst_assoc) (oid\<^sub>P\<^sub>e\<^sub>r\<^sub>s\<^sub>o\<^sub>n_0_\<B>\<O>\<S>\<S>) (switch\<^sub>2_01) (oid1))) (\<lfloor>1300\<rfloor>))"
-definition "X\<^sub>P\<^sub>e\<^sub>r\<^sub>s\<^sub>o\<^sub>n2\<^sub>P\<^sub>e\<^sub>r\<^sub>s\<^sub>o\<^sub>n inst_assoc = (mkoid\<^sub>P\<^sub>e\<^sub>r\<^sub>s\<^sub>o\<^sub>n ((mk\<^sub>P\<^sub>e\<^sub>r\<^sub>s\<^sub>o\<^sub>n (oid2) (None) (None) (None) (None) (None))) (((inst_assoc) (oid\<^sub>P\<^sub>e\<^sub>r\<^sub>s\<^sub>o\<^sub>n_0_\<B>\<O>\<S>\<S>) (switch\<^sub>2_01) (oid2))) (\<lfloor>1800\<rfloor>))"
-definition "X\<^sub>P\<^sub>e\<^sub>r\<^sub>s\<^sub>o\<^sub>n3\<^sub>P\<^sub>e\<^sub>r\<^sub>s\<^sub>o\<^sub>n inst_assoc = (mkoid\<^sub>P\<^sub>e\<^sub>r\<^sub>s\<^sub>o\<^sub>n ((mk\<^sub>P\<^sub>e\<^sub>r\<^sub>s\<^sub>o\<^sub>n (oid3) (None) (None) (None) (None) (None))) (((inst_assoc) (oid\<^sub>P\<^sub>e\<^sub>r\<^sub>s\<^sub>o\<^sub>n_0_\<B>\<O>\<S>\<S>) (switch\<^sub>2_01) (oid3))) (None))"
-definition "X\<^sub>P\<^sub>e\<^sub>r\<^sub>s\<^sub>o\<^sub>n4\<^sub>P\<^sub>e\<^sub>r\<^sub>s\<^sub>o\<^sub>n inst_assoc = (mkoid\<^sub>P\<^sub>e\<^sub>r\<^sub>s\<^sub>o\<^sub>n ((mk\<^sub>P\<^sub>e\<^sub>r\<^sub>s\<^sub>o\<^sub>n (oid4) (None) (None) (None) (None) (None))) (((inst_assoc) (oid\<^sub>P\<^sub>e\<^sub>r\<^sub>s\<^sub>o\<^sub>n_0_\<B>\<O>\<S>\<S>) (switch\<^sub>2_01) (oid4))) (\<lfloor>2900\<rfloor>))"
-definition "X\<^sub>P\<^sub>e\<^sub>r\<^sub>s\<^sub>o\<^sub>n5\<^sub>P\<^sub>e\<^sub>r\<^sub>s\<^sub>o\<^sub>n inst_assoc = (mkoid\<^sub>P\<^sub>e\<^sub>r\<^sub>s\<^sub>o\<^sub>n ((mk\<^sub>P\<^sub>e\<^sub>r\<^sub>s\<^sub>o\<^sub>n (oid5) (None) (None) (None) (None) (None))) (((inst_assoc) (oid\<^sub>P\<^sub>e\<^sub>r\<^sub>s\<^sub>o\<^sub>n_0_\<B>\<O>\<S>\<S>) (switch\<^sub>2_01) (oid5))) (\<lfloor>3500\<rfloor>))"
-definition "X\<^sub>P\<^sub>e\<^sub>r\<^sub>s\<^sub>o\<^sub>n6\<^sub>P\<^sub>e\<^sub>r\<^sub>s\<^sub>o\<^sub>n inst_assoc = (mkoid\<^sub>P\<^sub>e\<^sub>r\<^sub>s\<^sub>o\<^sub>n ((mk\<^sub>P\<^sub>e\<^sub>r\<^sub>s\<^sub>o\<^sub>n (oid6) (None) (None) (None) (None) (None))) (((inst_assoc) (oid\<^sub>P\<^sub>e\<^sub>r\<^sub>s\<^sub>o\<^sub>n_0_\<B>\<O>\<S>\<S>) (switch\<^sub>2_01) (oid6))) (\<lfloor>2500\<rfloor>))"
-definition "X\<^sub>P\<^sub>e\<^sub>r\<^sub>s\<^sub>o\<^sub>n7\<^sub>O\<^sub>c\<^sub>l\<^sub>A\<^sub>n\<^sub>y inst_assoc = (mkoid\<^sub>O\<^sub>c\<^sub>l\<^sub>A\<^sub>n\<^sub>y ((mk\<^sub>O\<^sub>c\<^sub>l\<^sub>A\<^sub>n\<^sub>y_\<^sub>P\<^sub>e\<^sub>r\<^sub>s\<^sub>o\<^sub>n ((mkoid\<^sub>P\<^sub>e\<^sub>r\<^sub>s\<^sub>o\<^sub>n ((mk\<^sub>P\<^sub>e\<^sub>r\<^sub>s\<^sub>o\<^sub>n (oid7) (None) (None) (None) (None) (None))) (((inst_assoc) (oid\<^sub>P\<^sub>e\<^sub>r\<^sub>s\<^sub>o\<^sub>n_0_\<B>\<O>\<S>\<S>) (switch\<^sub>2_01) (oid7))) (\<lfloor>3200\<rfloor>))))))"
-definition "X\<^sub>P\<^sub>e\<^sub>r\<^sub>s\<^sub>o\<^sub>n8\<^sub>O\<^sub>c\<^sub>l\<^sub>A\<^sub>n\<^sub>y inst_assoc = (mkoid\<^sub>O\<^sub>c\<^sub>l\<^sub>A\<^sub>n\<^sub>y ((mk\<^sub>O\<^sub>c\<^sub>l\<^sub>A\<^sub>n\<^sub>y (oid8))))"
-definition "X\<^sub>P\<^sub>e\<^sub>r\<^sub>s\<^sub>o\<^sub>n9\<^sub>P\<^sub>e\<^sub>r\<^sub>s\<^sub>o\<^sub>n inst_assoc = (mkoid\<^sub>P\<^sub>e\<^sub>r\<^sub>s\<^sub>o\<^sub>n ((mk\<^sub>P\<^sub>e\<^sub>r\<^sub>s\<^sub>o\<^sub>n (oid9) (None) (None) (None) (None) (None))) (((inst_assoc) (oid\<^sub>P\<^sub>e\<^sub>r\<^sub>s\<^sub>o\<^sub>n_0_\<B>\<O>\<S>\<S>) (switch\<^sub>2_01) (oid9))) (\<lfloor>0\<rfloor>))"
-definition "X0\<^sub>P\<^sub>e\<^sub>r\<^sub>s\<^sub>o\<^sub>n inst_assoc = (mkoid\<^sub>P\<^sub>e\<^sub>r\<^sub>s\<^sub>o\<^sub>n ((mk\<^sub>P\<^sub>e\<^sub>r\<^sub>s\<^sub>o\<^sub>n (oid10) (None) (None) (None) (None) (\<lfloor>[[oid11]]\<rfloor>))) (((inst_assoc) (oid\<^sub>P\<^sub>e\<^sub>r\<^sub>s\<^sub>o\<^sub>n_0_\<B>\<O>\<S>\<S>) (switch\<^sub>2_01) (oid10))) (None))"
-definition "P1\<^sub>P\<^sub>l\<^sub>a\<^sub>n\<^sub>e\<^sub>t inst_assoc = (mkoid\<^sub>P\<^sub>l\<^sub>a\<^sub>n\<^sub>e\<^sub>t ((mk\<^sub>P\<^sub>l\<^sub>a\<^sub>n\<^sub>e\<^sub>t (oid11) (None) (None) (\<lfloor>[[oid11] , [oid11]]\<rfloor>))) (None) (None))"
+definition "X\<^sub>P\<^sub>e\<^sub>r\<^sub>s\<^sub>o\<^sub>n1\<^sub>P\<^sub>e\<^sub>r\<^sub>s\<^sub>o\<^sub>n inst_assoc = (mk\<^sub>P\<^sub>e\<^sub>r\<^sub>s\<^sub>o\<^sub>n ((mk\<E>\<X>\<T>\<^sub>P\<^sub>e\<^sub>r\<^sub>s\<^sub>o\<^sub>n (oid1) (None) (None) (None) (None) (None))) (((inst_assoc) (oid\<^sub>P\<^sub>e\<^sub>r\<^sub>s\<^sub>o\<^sub>n_0_\<B>\<O>\<S>\<S>) (switch\<^sub>2_01) (oid1))) (\<lfloor>1300\<rfloor>))"
+definition "X\<^sub>P\<^sub>e\<^sub>r\<^sub>s\<^sub>o\<^sub>n2\<^sub>P\<^sub>e\<^sub>r\<^sub>s\<^sub>o\<^sub>n inst_assoc = (mk\<^sub>P\<^sub>e\<^sub>r\<^sub>s\<^sub>o\<^sub>n ((mk\<E>\<X>\<T>\<^sub>P\<^sub>e\<^sub>r\<^sub>s\<^sub>o\<^sub>n (oid2) (None) (None) (None) (None) (None))) (((inst_assoc) (oid\<^sub>P\<^sub>e\<^sub>r\<^sub>s\<^sub>o\<^sub>n_0_\<B>\<O>\<S>\<S>) (switch\<^sub>2_01) (oid2))) (\<lfloor>1800\<rfloor>))"
+definition "X\<^sub>P\<^sub>e\<^sub>r\<^sub>s\<^sub>o\<^sub>n3\<^sub>P\<^sub>e\<^sub>r\<^sub>s\<^sub>o\<^sub>n inst_assoc = (mk\<^sub>P\<^sub>e\<^sub>r\<^sub>s\<^sub>o\<^sub>n ((mk\<E>\<X>\<T>\<^sub>P\<^sub>e\<^sub>r\<^sub>s\<^sub>o\<^sub>n (oid3) (None) (None) (None) (None) (None))) (((inst_assoc) (oid\<^sub>P\<^sub>e\<^sub>r\<^sub>s\<^sub>o\<^sub>n_0_\<B>\<O>\<S>\<S>) (switch\<^sub>2_01) (oid3))) (None))"
+definition "X\<^sub>P\<^sub>e\<^sub>r\<^sub>s\<^sub>o\<^sub>n4\<^sub>P\<^sub>e\<^sub>r\<^sub>s\<^sub>o\<^sub>n inst_assoc = (mk\<^sub>P\<^sub>e\<^sub>r\<^sub>s\<^sub>o\<^sub>n ((mk\<E>\<X>\<T>\<^sub>P\<^sub>e\<^sub>r\<^sub>s\<^sub>o\<^sub>n (oid4) (None) (None) (None) (None) (None))) (((inst_assoc) (oid\<^sub>P\<^sub>e\<^sub>r\<^sub>s\<^sub>o\<^sub>n_0_\<B>\<O>\<S>\<S>) (switch\<^sub>2_01) (oid4))) (\<lfloor>2900\<rfloor>))"
+definition "X\<^sub>P\<^sub>e\<^sub>r\<^sub>s\<^sub>o\<^sub>n5\<^sub>P\<^sub>e\<^sub>r\<^sub>s\<^sub>o\<^sub>n inst_assoc = (mk\<^sub>P\<^sub>e\<^sub>r\<^sub>s\<^sub>o\<^sub>n ((mk\<E>\<X>\<T>\<^sub>P\<^sub>e\<^sub>r\<^sub>s\<^sub>o\<^sub>n (oid5) (None) (None) (None) (None) (None))) (((inst_assoc) (oid\<^sub>P\<^sub>e\<^sub>r\<^sub>s\<^sub>o\<^sub>n_0_\<B>\<O>\<S>\<S>) (switch\<^sub>2_01) (oid5))) (\<lfloor>3500\<rfloor>))"
+definition "X\<^sub>P\<^sub>e\<^sub>r\<^sub>s\<^sub>o\<^sub>n6\<^sub>P\<^sub>e\<^sub>r\<^sub>s\<^sub>o\<^sub>n inst_assoc = (mk\<^sub>P\<^sub>e\<^sub>r\<^sub>s\<^sub>o\<^sub>n ((mk\<E>\<X>\<T>\<^sub>P\<^sub>e\<^sub>r\<^sub>s\<^sub>o\<^sub>n (oid6) (None) (None) (None) (None) (None))) (((inst_assoc) (oid\<^sub>P\<^sub>e\<^sub>r\<^sub>s\<^sub>o\<^sub>n_0_\<B>\<O>\<S>\<S>) (switch\<^sub>2_01) (oid6))) (\<lfloor>2500\<rfloor>))"
+definition "X\<^sub>P\<^sub>e\<^sub>r\<^sub>s\<^sub>o\<^sub>n7\<^sub>O\<^sub>c\<^sub>l\<^sub>A\<^sub>n\<^sub>y inst_assoc = (mk\<^sub>O\<^sub>c\<^sub>l\<^sub>A\<^sub>n\<^sub>y ((mk\<E>\<X>\<T>\<^sub>O\<^sub>c\<^sub>l\<^sub>A\<^sub>n\<^sub>y_\<^sub>P\<^sub>e\<^sub>r\<^sub>s\<^sub>o\<^sub>n ((mk\<^sub>P\<^sub>e\<^sub>r\<^sub>s\<^sub>o\<^sub>n ((mk\<E>\<X>\<T>\<^sub>P\<^sub>e\<^sub>r\<^sub>s\<^sub>o\<^sub>n (oid7) (None) (None) (None) (None) (None))) (((inst_assoc) (oid\<^sub>P\<^sub>e\<^sub>r\<^sub>s\<^sub>o\<^sub>n_0_\<B>\<O>\<S>\<S>) (switch\<^sub>2_01) (oid7))) (\<lfloor>3200\<rfloor>))))))"
+definition "X\<^sub>P\<^sub>e\<^sub>r\<^sub>s\<^sub>o\<^sub>n8\<^sub>O\<^sub>c\<^sub>l\<^sub>A\<^sub>n\<^sub>y inst_assoc = (mk\<^sub>O\<^sub>c\<^sub>l\<^sub>A\<^sub>n\<^sub>y ((mk\<E>\<X>\<T>\<^sub>O\<^sub>c\<^sub>l\<^sub>A\<^sub>n\<^sub>y (oid8))))"
+definition "X\<^sub>P\<^sub>e\<^sub>r\<^sub>s\<^sub>o\<^sub>n9\<^sub>P\<^sub>e\<^sub>r\<^sub>s\<^sub>o\<^sub>n inst_assoc = (mk\<^sub>P\<^sub>e\<^sub>r\<^sub>s\<^sub>o\<^sub>n ((mk\<E>\<X>\<T>\<^sub>P\<^sub>e\<^sub>r\<^sub>s\<^sub>o\<^sub>n (oid9) (None) (None) (None) (None) (None))) (((inst_assoc) (oid\<^sub>P\<^sub>e\<^sub>r\<^sub>s\<^sub>o\<^sub>n_0_\<B>\<O>\<S>\<S>) (switch\<^sub>2_01) (oid9))) (\<lfloor>0\<rfloor>))"
+definition "X0\<^sub>P\<^sub>e\<^sub>r\<^sub>s\<^sub>o\<^sub>n inst_assoc = (mk\<^sub>P\<^sub>e\<^sub>r\<^sub>s\<^sub>o\<^sub>n ((mk\<E>\<X>\<T>\<^sub>P\<^sub>e\<^sub>r\<^sub>s\<^sub>o\<^sub>n (oid10) (None) (None) (None) (None) (\<lfloor>[[oid11]]\<rfloor>))) (((inst_assoc) (oid\<^sub>P\<^sub>e\<^sub>r\<^sub>s\<^sub>o\<^sub>n_0_\<B>\<O>\<S>\<S>) (switch\<^sub>2_01) (oid10))) (None))"
+definition "P1\<^sub>P\<^sub>l\<^sub>a\<^sub>n\<^sub>e\<^sub>t inst_assoc = (mk\<^sub>P\<^sub>l\<^sub>a\<^sub>n\<^sub>e\<^sub>t ((mk\<E>\<X>\<T>\<^sub>P\<^sub>l\<^sub>a\<^sub>n\<^sub>e\<^sub>t (oid11) (None) (None) (\<lfloor>[[oid11] , [oid11]]\<rfloor>))) (None) (None))"
 definition "(X\<^sub>P\<^sub>e\<^sub>r\<^sub>s\<^sub>o\<^sub>n1::Person) = (\<lambda>_. \<lfloor>\<lfloor>(X\<^sub>P\<^sub>e\<^sub>r\<^sub>s\<^sub>o\<^sub>n1\<^sub>P\<^sub>e\<^sub>r\<^sub>s\<^sub>o\<^sub>n (inst_assoc1))\<rfloor>\<rfloor>)"
 definition "(X\<^sub>P\<^sub>e\<^sub>r\<^sub>s\<^sub>o\<^sub>n2::Person) = (\<lambda>_. \<lfloor>\<lfloor>(X\<^sub>P\<^sub>e\<^sub>r\<^sub>s\<^sub>o\<^sub>n2\<^sub>P\<^sub>e\<^sub>r\<^sub>s\<^sub>o\<^sub>n (inst_assoc1))\<rfloor>\<rfloor>)"
 definition "(X\<^sub>P\<^sub>e\<^sub>r\<^sub>s\<^sub>o\<^sub>n3::Person) = (\<lambda>_. \<lfloor>\<lfloor>(X\<^sub>P\<^sub>e\<^sub>r\<^sub>s\<^sub>o\<^sub>n3\<^sub>P\<^sub>e\<^sub>r\<^sub>s\<^sub>o\<^sub>n (inst_assoc1))\<rfloor>\<rfloor>)"
